<?xml version="1.0"?>
<rdf:RDF xmlns="https://w3id.org/icon/ontology/"
     xml:base="https://w3id.org/icon/ontology/"
     xmlns:dc="http://purl.org/dc/elements/1.1/"
     xmlns:crm="http://erlangen-crm.org/current/"
     xmlns:dct="https://www.w3.org/1999/xhtml/vocab#dct:"
     xmlns:dul="http://www.ontologydesignpatterns.org/ont/dul/DUL.owl#"
     xmlns:owl="http://www.w3.org/2002/07/owl#"
     xmlns:rdf="http://www.w3.org/1999/02/22-rdf-syntax-ns#"
     xmlns:xml="http://www.w3.org/XML/1998/namespace"
     xmlns:xsd="http://www.w3.org/2001/XMLSchema#"
     xmlns:icon="https://w3id.org/icon/ontology/"
     xmlns:rdfs="http://www.w3.org/2000/01/rdf-schema#"
     xmlns:skos="http://www.w3.org/2004/02/skos/core#"
     xmlns:vann="http://purl.org/vocab/vann/"
     xmlns:vocab="https://www.w3.org/1999/xhtml/vocab#"
     xmlns:schema="http://schema.org/"
     xmlns:dcterms="http://purl.org/dc/terms/"
     xmlns:cpannotationschema="http://www.ontologydesignpatterns.org/schemas/cpannotationschema.owl#">
    <owl:Ontology rdf:about="https://w3id.org/icon/ontology/">
        <owl:versionIRI rdf:resource="https://w3id.org/icon/ontology/1.1.0/"/>
        <owl:imports rdf:resource="http://erlangen-crm.org/current/"/>
        <owl:imports rdf:resource="http://purl.org/emmedi/hico/2020-03-31"/>
        <owl:imports rdf:resource="http://www.ontologydesignpatterns.org/ont/dul/DUL.owl"/>
        <owl:imports rdf:resource="http://www.w3.org/2004/02/skos/core"/>
        <owl:imports rdf:resource="https://www.w3id.org/simulation/ontology/"/>
        <dc:contributor xml:lang="en">Aldo Gangemi</dc:contributor>
        <dc:contributor xml:lang="en">Marieke van Erp</dc:contributor>
        <dc:creator>Bruno Sartini</dc:creator>
        <dc:creator>Sofia Baroncini</dc:creator>
        <dcterms:created xml:lang="en">April 12th, 2022</dcterms:created>
        <dcterms:issued xml:lang="en">April 12th, 2022</dcterms:issued>
        <dcterms:license xml:lang="en">https://creativecommons.org/licenses/by/4.0/</dcterms:license>
        <dcterms:publisher xml:lang="en">Bruno Sartini</dcterms:publisher>
        <dcterms:title xml:lang="en">ICON Ontology</dcterms:title>
        <vann:preferredNamespacePrefix xml:lang="en">icon</vann:preferredNamespacePrefix>
        <vann:preferredNamespaceUri xml:lang="en">https://w3id.org/icon/ontology/</vann:preferredNamespaceUri>
        <schema:citation xml:lang="en">Sartini B. and Baroncini S. Icon Ontology. https://w3id.org/icon/ontology</schema:citation>
        <rdfs:comment xml:lang="en">The ICON ontology deals with high granularity art interpretation. It was developed by conceptualizing Panofsky&apos;s theory of levels of interpretation, therefore artworks can be described according to Pre-iconographical, Iconographical and Iconological information.</rdfs:comment>
        <owl:backwardCompatibleWith xml:lang="en">First version</owl:backwardCompatibleWith>
        <owl:priorVersion xml:lang="en">1.0</owl:priorVersion>
        <owl:versionInfo xml:lang="en">1.1.0</owl:versionInfo>
    </owl:Ontology>
    


    <!-- 
    ///////////////////////////////////////////////////////////////////////////////////////
    //
    // Annotation properties
    //
    ///////////////////////////////////////////////////////////////////////////////////////
     -->

    


    <!-- http://purl.org/dc/terms/created -->

    <owl:AnnotationProperty rdf:about="http://purl.org/dc/terms/created"/>
    


    <!-- http://purl.org/dc/terms/issued -->

    <owl:AnnotationProperty rdf:about="http://purl.org/dc/terms/issued"/>
    


    <!-- http://purl.org/dc/terms/license -->

    <owl:AnnotationProperty rdf:about="http://purl.org/dc/terms/license"/>
    


    <!-- http://purl.org/dc/terms/title -->

    <owl:AnnotationProperty rdf:about="http://purl.org/dc/terms/title"/>
    


    <!-- http://www.w3.org/2001/XMLSchema#citation -->

    <owl:AnnotationProperty rdf:about="http://www.w3.org/2001/XMLSchema#citation"/>
    


    <!-- 
    ///////////////////////////////////////////////////////////////////////////////////////
    //
    // Object Properties
    //
    ///////////////////////////////////////////////////////////////////////////////////////
     -->

    


    <!-- http://purl.org/spar/cito/citesAsEvidence -->

    <owl:ObjectProperty rdf:about="http://purl.org/spar/cito/citesAsEvidence">
        <rdfs:domain rdf:resource="https://w3id.org/icon/ontology/Recognition"/>
    </owl:ObjectProperty>
    


    <!-- http://purl.org/spar/cito/citesForInformation -->

    <owl:ObjectProperty rdf:about="http://purl.org/spar/cito/citesForInformation">
        <rdfs:domain rdf:resource="https://w3id.org/icon/ontology/Recognition"/>
    </owl:ObjectProperty>
    


    <!-- http://purl.org/spar/cito/givesSupportTo -->

    <owl:ObjectProperty rdf:about="http://purl.org/spar/cito/givesSupportTo">
        <rdfs:domain rdf:resource="https://w3id.org/icon/ontology/Recognition"/>
        <rdfs:range rdf:resource="https://w3id.org/icon/ontology/Recognition"/>
    </owl:ObjectProperty>
    


    <!-- http://w3id.org/vir#K4_is_visual_prototype_of -->

    <owl:ObjectProperty rdf:about="http://w3id.org/vir#K4_is_visual_prototype_of"/>
    


    <!-- https://w3id.org/icon/ontology/aboutWorkOfArt -->

    <owl:ObjectProperty rdf:about="https://w3id.org/icon/ontology/aboutWorkOfArt">
        <owl:inverseOf rdf:resource="https://w3id.org/icon/ontology/interpretedByRecognition"/>
        <rdfs:domain rdf:resource="https://w3id.org/icon/ontology/Recognition"/>
        <rdfs:range rdf:resource="https://w3id.org/icon/ontology/Artwork"/>
        <rdfs:comment xml:lang="en">This relation associates each Recognition directly to the artwork. In this way, it is possible to retrieve easily all the interpretations about an artwork. Therefore, it a highly recommended good practice to declare it for each interpretation.</rdfs:comment>
        <rdfs:isDefinedBy rdf:resource="https://w3id.org/icon/ontology/ICONOntology"/>
        <rdfs:label xml:lang="en">About Work Of Art</rdfs:label>
    </owl:ObjectProperty>
    


    <!-- https://w3id.org/icon/ontology/associatedForm -->

    <owl:ObjectProperty rdf:about="https://w3id.org/icon/ontology/associatedForm">
        <rdfs:subPropertyOf rdf:resource="http://erlangen-crm.org/current/P140_assigned_attribute_to"/>
        <owl:inverseOf rdf:resource="https://w3id.org/icon/ontology/isPureFormOf"/>
        <rdfs:domain rdf:resource="https://w3id.org/icon/ontology/PreiconographicalRecognition"/>
        <rdfs:range rdf:resource="https://w3id.org/icon/ontology/PureForm"/>
        <rdfs:comment>This relation associates a Pure Form to the Pre-iconographical Recognition that describes it at the first level of interpretation.</rdfs:comment>
        <rdfs:label xml:lang="en">Associated Form</rdfs:label>
        <owl:deprecated>Since 1.1 version</owl:deprecated>
    </owl:ObjectProperty>
    


    <!-- https://w3id.org/icon/ontology/composedOf -->

    <owl:ObjectProperty rdf:about="https://w3id.org/icon/ontology/composedOf">
        <owl:inverseOf rdf:resource="https://w3id.org/icon/ontology/takesPartIn"/>
        <rdfs:domain rdf:resource="https://w3id.org/icon/ontology/Invenzione"/>
        <rdfs:range>
            <owl:Class>
                <owl:unionOf rdf:parseType="Collection">
                    <rdf:Description rdf:about="https://w3id.org/icon/ontology/Character"/>
                    <rdf:Description rdf:about="https://w3id.org/icon/ontology/Event"/>
                    <rdf:Description rdf:about="https://w3id.org/icon/ontology/NamedObject"/>
                    <rdf:Description rdf:about="https://w3id.org/icon/ontology/Personification"/>
                    <rdf:Description rdf:about="https://w3id.org/icon/ontology/Place"/>
                    <rdf:Description rdf:about="https://w3id.org/icon/ontology/Symbol"/>
                </owl:unionOf>
            </owl:Class>
        </rdfs:range>
        <rdfs:comment xml:lang="en">This Property links an invenzione with its components, which may vary from Characters, Events, Named Objects, Places to Personifications, Symbols according to the kind of Invenzione is being described.</rdfs:comment>
        <rdfs:isDefinedBy rdf:resource="https://w3id.org/icon/ontology/ICONOntology"/>
        <rdfs:label xml:lang="en">Composed Of</rdfs:label>
    </owl:ObjectProperty>
    


    <!-- https://w3id.org/icon/ontology/hasArtisticMotif -->

    <owl:ObjectProperty rdf:about="https://w3id.org/icon/ontology/hasArtisticMotif">
        <owl:inverseOf rdf:resource="https://w3id.org/icon/ontology/isArtisticMotifOf"/>
        <rdfs:domain rdf:resource="https://w3id.org/icon/ontology/IntrinsicMeaning"/>
        <rdfs:range rdf:resource="https://w3id.org/icon/ontology/ArtisticMotif"/>
        <rdfs:comment xml:lang="en">This relation links an Intrinsic Meaning to the Artistic Motif recognized at the first level of interpretation. It should be used to express that the third level meaning associated to the Intrinsic Meaning refers specifically to this Artistic Motif, and not only to the general artwork.</rdfs:comment>
        <rdfs:isDefinedBy rdf:resource="https://w3id.org/icon/ontology/ICONOntology"/>
        <rdfs:label xml:lang="en">Has Artistic Motif</rdfs:label>
    </owl:ObjectProperty>
    


    <!-- https://w3id.org/icon/ontology/hasCharacter -->

    <owl:ObjectProperty rdf:about="https://w3id.org/icon/ontology/hasCharacter">
        <owl:inverseOf rdf:resource="https://w3id.org/icon/ontology/isCharacterOf"/>
        <rdfs:domain rdf:resource="https://w3id.org/icon/ontology/Image"/>
        <rdfs:range rdf:resource="https://w3id.org/icon/ontology/Character"/>
        <skos:broadMatch rdf:resource="http://erlangen-crm.org/current/P138_represents"/>
    </owl:ObjectProperty>
    


    <!-- https://w3id.org/icon/ontology/hasComposition -->

    <owl:ObjectProperty rdf:about="https://w3id.org/icon/ontology/hasComposition">
        <owl:inverseOf rdf:resource="https://w3id.org/icon/ontology/isCompositionOf"/>
        <rdfs:domain rdf:resource="https://w3id.org/icon/ontology/IntrinsicMeaning"/>
        <rdfs:range rdf:resource="https://w3id.org/icon/ontology/Composition"/>
        <rdfs:comment xml:lang="en">This relation links an Intrinsic Meaning to the Composition recognized at the first level of interpretation. It should be used to express that the third level meaning associated to the Intrinsic Meaning refers specifically to this Composition, and not only to the general artwork.</rdfs:comment>
        <rdfs:isDefinedBy rdf:resource="https://w3id.org/icon/ontology/ICONOntology"/>
        <rdfs:label xml:lang="en">Has Composition</rdfs:label>
    </owl:ObjectProperty>
    


    <!-- https://w3id.org/icon/ontology/hasCompositionalStructure -->

    <owl:ObjectProperty rdf:about="https://w3id.org/icon/ontology/hasCompositionalStructure">
        <owl:inverseOf rdf:resource="https://w3id.org/icon/ontology/isCompositionalStructureOf"/>
        <rdfs:domain rdf:resource="https://w3id.org/icon/ontology/Composition"/>
        <rdfs:range rdf:resource="https://w3id.org/icon/ontology/CompositionalStructure"/>
        <rdfs:comment>This relation describes the arrangement of the Artistic Motifs composing the Composition. It is suggested to use it only when they are arranged in a relevant observable structure (e.g. pyramidal, oblique)</rdfs:comment>
        <rdfs:isDefinedBy rdf:resource="https://w3id.org/icon/ontology/ICONOntology"/>
        <rdfs:label xml:lang="en">Has Compositional Structure</rdfs:label>
    </owl:ObjectProperty>
    


    <!-- https://w3id.org/icon/ontology/hasCopiedMotif -->

    <owl:ObjectProperty rdf:about="https://w3id.org/icon/ontology/hasCopiedMotif">
        <owl:inverseOf rdf:resource="https://w3id.org/icon/ontology/isCopiedMotifOf"/>
        <rdfs:domain rdf:resource="https://w3id.org/icon/ontology/FormalMotifRecognition"/>
        <rdfs:range>
            <owl:Class>
                <owl:unionOf rdf:parseType="Collection">
                    <rdf:Description rdf:about="https://w3id.org/icon/ontology/ArtisticMotif"/>
                    <rdf:Description rdf:about="https://w3id.org/icon/ontology/Composition"/>
                </owl:unionOf>
            </owl:Class>
        </rdfs:range>
        <skos:broadMatch rdf:resource="http://w3id.org/vir#K4_is_visual_prototype_of"/>
    </owl:ObjectProperty>
    


    <!-- https://w3id.org/icon/ontology/hasEvent -->

    <owl:ObjectProperty rdf:about="https://w3id.org/icon/ontology/hasEvent">
        <owl:inverseOf rdf:resource="https://w3id.org/icon/ontology/isEventOf"/>
        <rdfs:domain rdf:resource="https://w3id.org/icon/ontology/Image"/>
        <rdfs:range rdf:resource="https://w3id.org/icon/ontology/Event"/>
        <skos:broadMatch rdf:resource="http://erlangen-crm.org/current/P138_represents"/>
    </owl:ObjectProperty>
    


    <!-- https://w3id.org/icon/ontology/hasExpressionalMeaning -->

    <owl:ObjectProperty rdf:about="https://w3id.org/icon/ontology/hasExpressionalMeaning">
        <owl:inverseOf rdf:resource="https://w3id.org/icon/ontology/isExpressionalMeaningOf"/>
        <rdfs:domain>
            <owl:Class>
                <owl:unionOf rdf:parseType="Collection">
                    <rdf:Description rdf:about="https://w3id.org/icon/ontology/ArtisticMotif"/>
                    <rdf:Description rdf:about="https://w3id.org/icon/ontology/Composition"/>
                </owl:unionOf>
            </owl:Class>
        </rdfs:domain>
        <rdfs:range rdf:resource="https://w3id.org/icon/ontology/ExpressionalQuality"/>
    <skos:broadMatch rdf:resource="http://erlangen-crm.org/current/P138_represents"/>
    </owl:ObjectProperty>
    


    <!-- https://w3id.org/icon/ontology/hasFactualMeaning -->

    <owl:ObjectProperty rdf:about="https://w3id.org/icon/ontology/hasFactualMeaning">
        <owl:inverseOf rdf:resource="https://w3id.org/icon/ontology/isFactualMeaningOf"/>
        <rdfs:domain>
            <owl:Class>
                <owl:unionOf rdf:parseType="Collection">
                    <rdf:Description rdf:about="https://w3id.org/icon/ontology/ArtisticMotif"/>
                    <rdf:Description rdf:about="https://w3id.org/icon/ontology/Composition"/>
                </owl:unionOf>
            </owl:Class>
        </rdfs:domain>
        <rdfs:range>
            <owl:Class>
                <owl:unionOf rdf:parseType="Collection">
                    <rdf:Description rdf:about="https://w3id.org/icon/ontology/Action"/>
                    <rdf:Description rdf:about="https://w3id.org/icon/ontology/NaturalElement"/>
                </owl:unionOf>
            </owl:Class>
        </rdfs:range>
        <skos:broadMatch rdf:resource="http://erlangen-crm.org/current/P138_represents"/>
    </owl:ObjectProperty>
    


    <!-- https://w3id.org/icon/ontology/hasImage -->

    <owl:ObjectProperty rdf:about="https://w3id.org/icon/ontology/hasImage">
        <owl:inverseOf rdf:resource="https://w3id.org/icon/ontology/isImageOf"/>
        <rdfs:domain rdf:resource="https://w3id.org/icon/ontology/IntrinsicMeaning"/>
        <rdfs:range rdf:resource="https://w3id.org/icon/ontology/Image"/>
        <rdfs:comment xml:lang="en">This relation links an Intrinsic Meaning to the Image recognized at the second level of interpretation. It should be used to express that the third level meaning associated to the Intrinsic Meaning refers specifically to this Image, and not only to the general artwork.</rdfs:comment>
        <rdfs:isDefinedBy rdf:resource="https://w3id.org/icon/ontology/ICONOntology"/>
        <rdfs:label xml:lang="en">Has Image</rdfs:label>
    </owl:ObjectProperty>
    


    <!-- https://w3id.org/icon/ontology/hasInvenzione -->

    <owl:ObjectProperty rdf:about="https://w3id.org/icon/ontology/hasInvenzione">
        <owl:inverseOf rdf:resource="https://w3id.org/icon/ontology/isInvenzioneOf"/>
        <rdfs:domain rdf:resource="https://w3id.org/icon/ontology/IntrinsicMeaning"/>
        <rdfs:range rdf:resource="https://w3id.org/icon/ontology/Invenzione"/>
        <rdfs:comment xml:lang="en">This relation links an Intrinsic Meaning to the Invenzione recognized at the second level of interpretation. It should be used to express that the third level meaning associated to the Intrinsic Meaning refers specifically to this invenzione, and not only to the general artwork.</rdfs:comment>
        <rdfs:isDefinedBy rdf:resource="https://w3id.org/icon/ontology/ICONOntology"/>
        <rdfs:label xml:lang="en">Has Invenzione</rdfs:label>
    </owl:ObjectProperty>
    


    <!-- https://w3id.org/icon/ontology/hasNamedObject -->

    <owl:ObjectProperty rdf:about="https://w3id.org/icon/ontology/hasNamedObject">
        <owl:inverseOf rdf:resource="https://w3id.org/icon/ontology/isNamedObjectOf"/>
        <rdfs:domain rdf:resource="https://w3id.org/icon/ontology/Image"/>
        <rdfs:range rdf:resource="https://w3id.org/icon/ontology/NamedObject"/>
        <skos:broadMatch rdf:resource="http://erlangen-crm.org/current/P138_represents"/>
    </owl:ObjectProperty>
    


    <!-- https://w3id.org/icon/ontology/hasPart -->

    <owl:ObjectProperty rdf:about="https://w3id.org/icon/ontology/hasPart">
        <rdfs:subPropertyOf rdf:resource="http://erlangen-crm.org/current/P106_is_composed_of"/>
        <rdfs:subPropertyOf rdf:resource="http://www.ontologydesignpatterns.org/ont/dul/DUL.owl#hasPart"/>
        <owl:inverseOf rdf:resource="https://w3id.org/icon/ontology/partOf"/>
        <rdfs:domain rdf:resource="https://w3id.org/icon/ontology/Composition"/>
        <rdfs:range rdf:resource="https://w3id.org/icon/ontology/ArtisticMotif"/>
        <rdfs:comment xml:lang="en">This relation links a Composition to the Artistic Motifs of which it consists.</rdfs:comment>
        <rdfs:label xml:lang="en">Has Part (ICON)</rdfs:label>
    </owl:ObjectProperty>
    


    <!-- https://w3id.org/icon/ontology/hasPersonification -->

    <owl:ObjectProperty rdf:about="https://w3id.org/icon/ontology/hasPersonification">
        <owl:inverseOf rdf:resource="https://w3id.org/icon/ontology/isPersonificationOf"/>
        <rdfs:domain rdf:resource="https://w3id.org/icon/ontology/Image"/>
        <rdfs:range rdf:resource="https://w3id.org/icon/ontology/Personification"/>
        <skos:broadMatch rdf:resource="http://erlangen-crm.org/current/P138_represents"/>
    </owl:ObjectProperty>
    


    <!-- https://w3id.org/icon/ontology/hasPlace -->

    <owl:ObjectProperty rdf:about="https://w3id.org/icon/ontology/hasPlace">
        <owl:inverseOf rdf:resource="https://w3id.org/icon/ontology/isPlaceOf"/>
        <rdfs:domain rdf:resource="https://w3id.org/icon/ontology/Image"/>
        <rdfs:range>
            <owl:Class>
                <owl:unionOf rdf:parseType="Collection">
                    <rdf:Description rdf:about="http://erlangen-crm.org/current/E53_Place"/>
                    <rdf:Description rdf:about="http://www.ontologydesignpatterns.org/ont/dul/DUL.owl#Place"/>
                </owl:unionOf>
            </owl:Class>
        </rdfs:range>
        <skos:broadMatch rdf:resource="http://erlangen-crm.org/current/P138_represents"/>
    </owl:ObjectProperty>
    


    <!-- https://w3id.org/icon/ontology/hasPrototypicalMotif -->

    <owl:ObjectProperty rdf:about="https://w3id.org/icon/ontology/hasPrototypicalMotif">
        <owl:inverseOf rdf:resource="https://w3id.org/icon/ontology/isPrototypicalMotifOf"/>
        <rdfs:domain rdf:resource="https://w3id.org/icon/ontology/FormalMotifRecognition"/>
        <rdfs:range>
            <owl:Class>
                <owl:unionOf rdf:parseType="Collection">
                    <rdf:Description rdf:about="https://w3id.org/icon/ontology/ArtisticMotif"/>
                    <rdf:Description rdf:about="https://w3id.org/icon/ontology/Composition"/>
                </owl:unionOf>
            </owl:Class>
        </rdfs:range>
        <skos:broadMatch rdf:resource="http://w3id.org/vir#K4_is_visual_prototype_of"/>
    </owl:ObjectProperty>
    


    <!-- https://w3id.org/icon/ontology/hasRecAttribute -->

    <owl:ObjectProperty rdf:about="https://w3id.org/icon/ontology/hasRecAttribute">
        <owl:inverseOf rdf:resource="https://w3id.org/icon/ontology/isRecAttributeOf"/>
        <rdfs:domain rdf:resource="https://w3id.org/icon/ontology/Image"/>
        <rdfs:range rdf:resource="https://w3id.org/icon/ontology/ArtisticMotif"/>
        <rdfs:comment xml:lang="en">This relation identifies objects belonging to the level 1 as fundamental for the recognition of a certain subject. It is suggested that the Artistic Motif of the object is included in the Composition corresponding to the subject.</rdfs:comment>
        <rdfs:isDefinedBy rdf:resource="https://w3id.org/icon/ontology/ICONOntology"/>
        <rdfs:label xml:lang="en">Has Rec Attribute</rdfs:label>
    </owl:ObjectProperty>
    


    <!-- https://w3id.org/icon/ontology/hasSymbol -->

    <owl:ObjectProperty rdf:about="https://w3id.org/icon/ontology/hasSymbol">
        <owl:inverseOf rdf:resource="https://w3id.org/icon/ontology/isSymbolOf"/>
        <rdfs:domain rdf:resource="https://w3id.org/icon/ontology/Image"/>
        <rdfs:range>
            <owl:Class>
                <owl:unionOf rdf:parseType="Collection">
                    <rdf:Description rdf:about="https://w3id.org/icon/ontology/Symbol"/>
                    <rdf:Description rdf:about="https://www.w3id.org/simulation/ontology/Simulation"/>
                </owl:unionOf>
            </owl:Class>
        </rdfs:range>
        <skos:broadMatch rdf:resource="http://erlangen-crm.org/current/P138_represents"/>
    </owl:ObjectProperty>
    


    <!-- https://w3id.org/icon/ontology/iconographicallyCompliesWith -->

    <owl:ObjectProperty rdf:about="https://w3id.org/icon/ontology/iconographicallyCompliesWith">
        <rdfs:subPropertyOf rdf:resource="http://www.ontologydesignpatterns.org/ont/dul/DUL.owl#satisfies"/>
        <owl:inverseOf rdf:resource="https://w3id.org/icon/ontology/isCompliantWithIconographicalRecognition"/>
        <rdfs:domain rdf:resource="https://w3id.org/icon/ontology/IconographicalRecognition"/>
        <rdfs:range rdf:resource="https://w3id.org/icon/ontology/InterpretationDescription"/>
        <rdfs:comment xml:lang="en">This property is used to link all the iconographical recognitions that take part in one or more interpretation(s), to that/those interpretation(s)</rdfs:comment>
        <rdfs:isDefinedBy rdf:resource="https://w3id.org/icon/ontology/ICONOntology"/>
        <rdfs:label xml:lang="en">iconographically complies with</rdfs:label>
    </owl:ObjectProperty>
    


    <!-- https://w3id.org/icon/ontology/iconologicallyCompliesWith -->

    <owl:ObjectProperty rdf:about="https://w3id.org/icon/ontology/iconologicallyCompliesWith">
        <rdfs:subPropertyOf rdf:resource="http://www.ontologydesignpatterns.org/ont/dul/DUL.owl#satisfies"/>
        <owl:inverseOf rdf:resource="https://w3id.org/icon/ontology/isCompliantWithIconologicalRecognition"/>
        <rdfs:domain rdf:resource="https://w3id.org/icon/ontology/IconologicalRecognition"/>
        <rdfs:range rdf:resource="https://w3id.org/icon/ontology/InterpretationDescription"/>
        <rdfs:comment xml:lang="en">This property is used to link all the iconological recognitions that take part in one or more interpretation(s), to that/those interpretation(s)</rdfs:comment>
        <rdfs:isDefinedBy rdf:resource="https://w3id.org/icon/ontology/ICONOntology"/>
        <rdfs:label xml:lang="en">iconologically complies with</rdfs:label>
    </owl:ObjectProperty>
    


    <!-- https://w3id.org/icon/ontology/interpretedByRecognition -->

    <owl:ObjectProperty rdf:about="https://w3id.org/icon/ontology/interpretedByRecognition">
        <rdfs:domain rdf:resource="https://w3id.org/icon/ontology/Artwork"/>
        <rdfs:range rdf:resource="https://w3id.org/icon/ontology/Recognition"/>
        <rdfs:comment xml:lang="en">Inverse property of aboutWorkOfArt</rdfs:comment>
        <rdfs:isDefinedBy rdf:resource="https://w3id.org/icon/ontology/ICONOntology"/>
        <rdfs:label xml:lang="en">Interpreted By Recognition</rdfs:label>
    </owl:ObjectProperty>
    


    <!-- https://w3id.org/icon/ontology/isArtisticMotifOf -->

    <owl:ObjectProperty rdf:about="https://w3id.org/icon/ontology/isArtisticMotifOf">
        <rdf:type rdf:resource="http://www.w3.org/2002/07/owl#FunctionalProperty"/>
        <rdfs:domain rdf:resource="https://w3id.org/icon/ontology/ArtisticMotif"/>
        <rdfs:range rdf:resource="https://w3id.org/icon/ontology/IntrinsicMeaning"/>
        <rdfs:comment>Inverse property of has artistic motif</rdfs:comment>
        <rdfs:isDefinedBy rdf:resource="https://w3id.org/icon/ontology/ICONOntology"/>
        <rdfs:label xml:lang="en">Is artistic motif of</rdfs:label>
    </owl:ObjectProperty>
    


    <!-- https://w3id.org/icon/ontology/isCharacterOf -->

    <owl:ObjectProperty rdf:about="https://w3id.org/icon/ontology/isCharacterOf">
        <rdfs:domain rdf:resource="https://w3id.org/icon/ontology/Character"/>
        <rdfs:range rdf:resource="https://w3id.org/icon/ontology/Image"/>
        <rdfs:comment xml:lang="en">Inverse property of hasCharacter</rdfs:comment>
        <rdfs:isDefinedBy rdf:resource="https://w3id.org/icon/ontology/ICONOntology"/>
        <rdfs:label xml:lang="en">Is Character Of</rdfs:label>
    </owl:ObjectProperty>
    


    <!-- https://w3id.org/icon/ontology/isCompliantWithIconographicalRecognition -->

    <owl:ObjectProperty rdf:about="https://w3id.org/icon/ontology/isCompliantWithIconographicalRecognition">
        <rdfs:subPropertyOf rdf:resource="http://www.ontologydesignpatterns.org/ont/dul/DUL.owl#isSatisfiedBy"/>
        <rdfs:domain rdf:resource="https://w3id.org/icon/ontology/InterpretationDescription"/>
        <rdfs:range rdf:resource="https://w3id.org/icon/ontology/IconographicalRecognition"/>
        <rdfs:comment xml:lang="en">Inverse of iconographically complies with</rdfs:comment>
        <rdfs:isDefinedBy rdf:resource="https://w3id.org/icon/ontology/ICONOntology"/>
        <rdfs:label xml:lang="en">is compliant with iconographical recognition</rdfs:label>
    </owl:ObjectProperty>
    


    <!-- https://w3id.org/icon/ontology/isCompliantWithIconologicalRecognition -->

    <owl:ObjectProperty rdf:about="https://w3id.org/icon/ontology/isCompliantWithIconologicalRecognition">
        <rdfs:subPropertyOf rdf:resource="http://www.ontologydesignpatterns.org/ont/dul/DUL.owl#isSatisfiedBy"/>
        <rdfs:domain rdf:resource="https://w3id.org/icon/ontology/InterpretationDescription"/>
        <rdfs:range rdf:resource="https://w3id.org/icon/ontology/PreiconographicalRecognition"/>
        <rdfs:comment xml:lang="en">inverse of iconologically complies with</rdfs:comment>
        <rdfs:isDefinedBy rdf:resource="https://w3id.org/icon/ontology/ICONOntology"/>
        <rdfs:label xml:lang="en">is compliant with iconological recognition</rdfs:label>
    </owl:ObjectProperty>
    


    <!-- https://w3id.org/icon/ontology/isCompliantWithPreiconographicalRecognition -->

    <owl:ObjectProperty rdf:about="https://w3id.org/icon/ontology/isCompliantWithPreiconographicalRecognition">
        <rdfs:subPropertyOf rdf:resource="http://www.ontologydesignpatterns.org/ont/dul/DUL.owl#isSatisfiedBy"/>
        <owl:inverseOf rdf:resource="https://w3id.org/icon/ontology/preiconographicallyCompliesWith"/>
        <rdfs:domain rdf:resource="https://w3id.org/icon/ontology/InterpretationDescription"/>
        <rdfs:range>
            <owl:Class>
                <owl:unionOf rdf:parseType="Collection">
                    <rdf:Description rdf:about="https://w3id.org/icon/ontology/FormalMotifRecognition"/>
                    <rdf:Description rdf:about="https://w3id.org/icon/ontology/PreiconographicalRecognition"/>
                </owl:unionOf>
            </owl:Class>
        </rdfs:range>
        <rdfs:comment xml:lang="en">Inverse of pre-iconographically complies with</rdfs:comment>
        <rdfs:isDefinedBy rdf:resource="https://w3id.org/icon/ontology/ICONOntology"/>
        <rdfs:label xml:lang="en">is compliant with pre-iconographical recognition</rdfs:label>
    </owl:ObjectProperty>
    


    <!-- https://w3id.org/icon/ontology/isCompositionOf -->

    <owl:ObjectProperty rdf:about="https://w3id.org/icon/ontology/isCompositionOf">
        <rdfs:domain rdf:resource="https://w3id.org/icon/ontology/Composition"/>
        <rdfs:range rdf:resource="https://w3id.org/icon/ontology/IntrinsicMeaning"/>
        <rdfs:comment xml:lang="en">Inverse property of has composition</rdfs:comment>
        <rdfs:isDefinedBy rdf:resource="https://w3id.org/icon/ontology/ICONOntology"/>
        <rdfs:label xml:lang="en">Is composition of</rdfs:label>
    </owl:ObjectProperty>
    


    <!-- https://w3id.org/icon/ontology/isCompositionalStructureOf -->

    <owl:ObjectProperty rdf:about="https://w3id.org/icon/ontology/isCompositionalStructureOf">
        <rdfs:domain rdf:resource="https://w3id.org/icon/ontology/CompositionalStructure"/>
        <rdfs:range rdf:resource="https://w3id.org/icon/ontology/Composition"/>
        <rdfs:comment xml:lang="en">Inverse property of hasCompositionalStructure</rdfs:comment>
        <rdfs:isDefinedBy rdf:resource="https://w3id.org/icon/ontology/ICONOntology"/>
        <rdfs:label xml:lang="en">Is Compositional Structure Of</rdfs:label>
    </owl:ObjectProperty>
    


    <!-- https://w3id.org/icon/ontology/isCopiedMotifOf -->

    <owl:ObjectProperty rdf:about="https://w3id.org/icon/ontology/isCopiedMotifOf">
        <rdfs:domain>
            <owl:Class>
                <owl:unionOf rdf:parseType="Collection">
                    <rdf:Description rdf:about="https://w3id.org/icon/ontology/ArtisticMotif"/>
                    <rdf:Description rdf:about="https://w3id.org/icon/ontology/Composition"/>
                </owl:unionOf>
            </owl:Class>
        </rdfs:domain>
        <rdfs:range rdf:resource="https://w3id.org/icon/ontology/FormalMotifRecognition"/>
        <rdfs:comment xml:lang="en">Inverse property of hasCopiedMotif</rdfs:comment>
        <rdfs:isDefinedBy rdf:resource="https://w3id.org/icon/ontology/ICONOntology"/>
        <rdfs:label xml:lang="en">Is Copied Motif Of</rdfs:label>
    </owl:ObjectProperty>
    


    <!-- https://w3id.org/icon/ontology/isCulturalPhenomenonOf -->

    <owl:ObjectProperty rdf:about="https://w3id.org/icon/ontology/isCulturalPhenomenonOf">
        <owl:inverseOf rdf:resource="https://w3id.org/icon/ontology/recognizedCulturalPhenomenon"/>
        <rdfs:domain rdf:resource="https://w3id.org/icon/ontology/CulturalPhenomenon"/>
        <rdfs:range rdf:resource="https://w3id.org/icon/ontology/IntrinsicMeaning"/>
        <rdfs:comment xml:lang="en">Inverse property of recognizedCulturalPhenomenon</rdfs:comment>
        <rdfs:isDefinedBy rdf:resource="https://w3id.org/icon/ontology/ICONOntology"/>
        <rdfs:label xml:lang="en">Is Cultural Phenomenon Of</rdfs:label>
    </owl:ObjectProperty>
    


    <!-- https://w3id.org/icon/ontology/isEventOf -->

    <owl:ObjectProperty rdf:about="https://w3id.org/icon/ontology/isEventOf">
        <rdfs:domain rdf:resource="https://w3id.org/icon/ontology/Event"/>
        <rdfs:range rdf:resource="https://w3id.org/icon/ontology/Image"/>
        <rdfs:comment xml:lang="en">Inverse property of hasEvent</rdfs:comment>
        <rdfs:isDefinedBy rdf:resource="https://w3id.org/icon/ontology/ICONOntology"/>
        <rdfs:label xml:lang="en">Is Event Of</rdfs:label>
    </owl:ObjectProperty>
    


    <!-- https://w3id.org/icon/ontology/isExpressionalMeaningOf -->

    <owl:ObjectProperty rdf:about="https://w3id.org/icon/ontology/isExpressionalMeaningOf">
        <rdfs:domain rdf:resource="https://w3id.org/icon/ontology/ExpressionalQuality"/>
        <rdfs:range>
            <owl:Class>
                <owl:unionOf rdf:parseType="Collection">
                    <rdf:Description rdf:about="https://w3id.org/icon/ontology/ArtisticMotif"/>
                    <rdf:Description rdf:about="https://w3id.org/icon/ontology/Composition"/>
                </owl:unionOf>
            </owl:Class>
        </rdfs:range>
        <rdfs:comment xml:lang="en">Inverse property of hasExpressionalMeaning</rdfs:comment>
        <rdfs:isDefinedBy rdf:resource="https://w3id.org/icon/ontology/ICONOntology"/>
        <rdfs:label xml:lang="en">Is Expressional Meaning Of</rdfs:label>
    </owl:ObjectProperty>
    


    <!-- https://w3id.org/icon/ontology/isFactualMeaningOf -->

    <owl:ObjectProperty rdf:about="https://w3id.org/icon/ontology/isFactualMeaningOf">
        <rdfs:domain>
            <owl:Class>
                <owl:unionOf rdf:parseType="Collection">
                    <rdf:Description rdf:about="https://w3id.org/icon/ontology/Action"/>
                    <rdf:Description rdf:about="https://w3id.org/icon/ontology/NaturalElement"/>
                </owl:unionOf>
            </owl:Class>
        </rdfs:domain>
        <rdfs:range>
            <owl:Class>
                <owl:unionOf rdf:parseType="Collection">
                    <rdf:Description rdf:about="https://w3id.org/icon/ontology/ArtisticMotif"/>
                    <rdf:Description rdf:about="https://w3id.org/icon/ontology/Composition"/>
                </owl:unionOf>
            </owl:Class>
        </rdfs:range>
        <rdfs:comment xml:lang="en">Inverse property of hasFactualMeaning</rdfs:comment>
        <rdfs:isDefinedBy rdf:resource="https://w3id.org/icon/ontology/ICONOntology"/>
        <rdfs:label xml:lang="en">Is Factual Meaning Of</rdfs:label>
    </owl:ObjectProperty>
    


    <!-- https://w3id.org/icon/ontology/isIconographicallyRecognizedBy -->

    <owl:ObjectProperty rdf:about="https://w3id.org/icon/ontology/isIconographicallyRecognizedBy">
        <owl:inverseOf rdf:resource="https://w3id.org/icon/ontology/recognizedImage"/>
        <rdfs:domain rdf:resource="https://w3id.org/icon/ontology/Image"/>
        <rdfs:range rdf:resource="https://w3id.org/icon/ontology/IconographicalRecognition"/>
        <rdfs:comment xml:lang="en">Inverse property of recognizedImage</rdfs:comment>
        <rdfs:isDefinedBy rdf:resource="https://w3id.org/icon/ontology/ICONOntology"/>
        <rdfs:label xml:lang="en">Is Iconographically Recognized By</rdfs:label>
    </owl:ObjectProperty>
    


    <!-- https://w3id.org/icon/ontology/isIconographicallyReferredBy -->

    <owl:ObjectProperty rdf:about="https://w3id.org/icon/ontology/isIconographicallyReferredBy">
        <owl:inverseOf rdf:resource="https://w3id.org/icon/ontology/refersToArtisticMotif"/>
        <rdfs:domain>
            <owl:Class>
                <owl:unionOf rdf:parseType="Collection">
                    <rdf:Description rdf:about="https://w3id.org/icon/ontology/ArtisticMotif"/>
                    <rdf:Description rdf:about="https://w3id.org/icon/ontology/Composition"/>
                </owl:unionOf>
            </owl:Class>
        </rdfs:domain>
        <rdfs:range rdf:resource="https://w3id.org/icon/ontology/IconographicalRecognition"/>
        <rdfs:comment rdf:datatype="http://www.w3.org/2000/01/rdf-schema#Literal">Inverse property of refers to artistic motif</rdfs:comment>
        <rdfs:isDefinedBy rdf:resource="https://w3id.org/icon/ontology/ICONOntology"/>
        <rdfs:label rdf:datatype="http://www.w3.org/2000/01/rdf-schema#Literal">Is iconographically referred by</rdfs:label>
    </owl:ObjectProperty>
    


    <!-- https://w3id.org/icon/ontology/isImageOf -->

    <owl:ObjectProperty rdf:about="https://w3id.org/icon/ontology/isImageOf">
        <rdfs:domain rdf:resource="https://w3id.org/icon/ontology/Image"/>
        <rdfs:range rdf:resource="https://w3id.org/icon/ontology/IntrinsicMeaning"/>
        <rdfs:comment xml:lang="en">Inverse property of has image</rdfs:comment>
        <rdfs:isDefinedBy rdf:resource="https://w3id.org/icon/ontology/ICONOntology"/>
        <rdfs:label xml:lang="en">Is image of</rdfs:label>
    </owl:ObjectProperty>
    


    <!-- https://w3id.org/icon/ontology/isIntrinsicMeaningOf -->

    <owl:ObjectProperty rdf:about="https://w3id.org/icon/ontology/isIntrinsicMeaningOf">
        <owl:inverseOf rdf:resource="https://w3id.org/icon/ontology/recognizedIntrinsicMeaning"/>
        <rdfs:domain rdf:resource="https://w3id.org/icon/ontology/IntrinsicMeaning"/>
        <rdfs:range rdf:resource="https://w3id.org/icon/ontology/IconologicalRecognition"/>
        <rdfs:comment xml:lang="en">Inverse property of recognized intrinsic meaning</rdfs:comment>
        <rdfs:isDefinedBy rdf:resource="https://w3id.org/icon/ontology/ICONOntology"/>
        <rdfs:label xml:lang="en">Is Intrinsic Meaning Of</rdfs:label>
    </owl:ObjectProperty>
    


    <!-- https://w3id.org/icon/ontology/isInvenzioneOf -->

    <owl:ObjectProperty rdf:about="https://w3id.org/icon/ontology/isInvenzioneOf">
        <rdfs:domain rdf:resource="https://w3id.org/icon/ontology/Invenzione"/>
        <rdfs:range rdf:resource="https://w3id.org/icon/ontology/IntrinsicMeaning"/>
        <rdfs:comment xml:lang="en">Inverse property of hasInvenzione</rdfs:comment>
        <rdfs:isDefinedBy rdf:resource="https://w3id.org/icon/ontology/ICONOntology"/>
        <rdfs:label xml:lang="en">Is Invenzione Of</rdfs:label>
    </owl:ObjectProperty>
    


    <!-- https://w3id.org/icon/ontology/isNamedObjectOf -->

    <owl:ObjectProperty rdf:about="https://w3id.org/icon/ontology/isNamedObjectOf">
        <rdfs:domain rdf:resource="https://w3id.org/icon/ontology/NamedObject"/>
        <rdfs:range rdf:resource="https://w3id.org/icon/ontology/Image"/>
        <rdfs:comment xml:lang="en">Inverse property of hasNamedObject</rdfs:comment>
        <rdfs:isDefinedBy rdf:resource="https://w3id.org/icon/ontology/ICONOntology"/>
        <rdfs:label xml:lang="en">Is Named Object Of</rdfs:label>
    </owl:ObjectProperty>
    


    <!-- https://w3id.org/icon/ontology/isPersonificationOf -->

    <owl:ObjectProperty rdf:about="https://w3id.org/icon/ontology/isPersonificationOf">
        <rdfs:domain rdf:resource="https://w3id.org/icon/ontology/Personification"/>
        <rdfs:range rdf:resource="https://w3id.org/icon/ontology/Image"/>
        <rdfs:comment xml:lang="en">Inverse property of hasPersonification</rdfs:comment>
        <rdfs:isDefinedBy rdf:resource="https://w3id.org/icon/ontology/ICONOntology"/>
        <rdfs:label xml:lang="en">Is Personification Of</rdfs:label>
    </owl:ObjectProperty>
    


    <!-- https://w3id.org/icon/ontology/isPlaceOf -->

    <owl:ObjectProperty rdf:about="https://w3id.org/icon/ontology/isPlaceOf">
        <rdfs:domain rdf:resource="http://www.ontologydesignpatterns.org/ont/dul/DUL.owl#Place"/>
        <rdfs:range rdf:resource="https://w3id.org/icon/ontology/Image"/>
        <rdfs:comment xml:lang="en">Inverse property of hasPlace</rdfs:comment>
        <rdfs:isDefinedBy rdf:resource="https://w3id.org/icon/ontology/ICONOntology"/>
        <rdfs:label xml:lang="en">Is Place Of</rdfs:label>
    </owl:ObjectProperty>
    


    <!-- https://w3id.org/icon/ontology/isPrototypicalMotifOf -->

    <owl:ObjectProperty rdf:about="https://w3id.org/icon/ontology/isPrototypicalMotifOf">
        <rdfs:domain>
            <owl:Class>
                <owl:unionOf rdf:parseType="Collection">
                    <rdf:Description rdf:about="https://w3id.org/icon/ontology/ArtisticMotif"/>
                    <rdf:Description rdf:about="https://w3id.org/icon/ontology/Composition"/>
                </owl:unionOf>
            </owl:Class>
        </rdfs:domain>
        <rdfs:range rdf:resource="https://w3id.org/icon/ontology/FormalMotifRecognition"/>
        <rdfs:comment xml:lang="en">Inverse property of hasPrototypicalMotif</rdfs:comment>
        <rdfs:isDefinedBy rdf:resource="https://w3id.org/icon/ontology/ICONOntology"/>
        <rdfs:label xml:lang="en">Is Prototypical Motif Of</rdfs:label>
    </owl:ObjectProperty>
    


    <!-- https://w3id.org/icon/ontology/isPureFormOf -->

    <owl:ObjectProperty rdf:about="https://w3id.org/icon/ontology/isPureFormOf">
        <rdfs:domain rdf:resource="https://w3id.org/icon/ontology/PureForm"/>
        <rdfs:range rdf:resource="https://w3id.org/icon/ontology/PreiconographicalRecognition"/>
        <rdfs:comment xml:lang="en">Inverse property of associatedForm</rdfs:comment>
        <rdfs:label xml:lang="en">Is Pure Form Of</rdfs:label>
        <owl:deprecated>since 1.1 version</owl:deprecated>
    </owl:ObjectProperty>
    


    <!-- https://w3id.org/icon/ontology/isRecAttributeOf -->

    <owl:ObjectProperty rdf:about="https://w3id.org/icon/ontology/isRecAttributeOf">
        <rdfs:domain rdf:resource="https://w3id.org/icon/ontology/ArtisticMotif"/>
        <rdfs:range rdf:resource="https://w3id.org/icon/ontology/Image"/>
        <rdfs:comment xml:lang="en">Inverse property of hasRecAttribute</rdfs:comment>
        <rdfs:isDefinedBy rdf:resource="https://w3id.org/icon/ontology/ICONOntology"/>
        <rdfs:label xml:lang="en">Is Rec Attribute Of</rdfs:label>
    </owl:ObjectProperty>
    


    <!-- https://w3id.org/icon/ontology/isRecognOf -->

    <owl:ObjectProperty rdf:about="https://w3id.org/icon/ontology/isRecognOf">
        <owl:inverseOf rdf:resource="https://w3id.org/icon/ontology/recognizedInvenzione"/>
        <rdfs:domain rdf:resource="https://w3id.org/icon/ontology/Invenzione"/>
        <rdfs:range rdf:resource="https://w3id.org/icon/ontology/IconographicalRecognition"/>
        <rdfs:comment xml:lang="en">Inverse property of recognizedInvenzione</rdfs:comment>
        <rdfs:isDefinedBy rdf:resource="https://w3id.org/icon/ontology/ICONOntology"/>
        <rdfs:label xml:lang="en">Is Recogn Of</rdfs:label>
    </owl:ObjectProperty>
    


    <!-- https://w3id.org/icon/ontology/isRecognizedArtisticMotifOf -->

    <owl:ObjectProperty rdf:about="https://w3id.org/icon/ontology/isRecognizedArtisticMotifOf">
        <owl:inverseOf rdf:resource="https://w3id.org/icon/ontology/recognizedArtisticMotif"/>
        <rdfs:domain rdf:resource="https://w3id.org/icon/ontology/ArtisticMotif"/>
        <rdfs:range rdf:resource="https://w3id.org/icon/ontology/PreiconographicalRecognition"/>
        <rdfs:comment xml:lang="en">Inverse property of recognized artistic motif</rdfs:comment>
        <rdfs:isDefinedBy rdf:resource="https://w3id.org/icon/ontology/ICONOntology"/>
        <rdfs:label xml:lang="en">Is Recognized Artistic Motif Of</rdfs:label>
    </owl:ObjectProperty>
    


    <!-- https://w3id.org/icon/ontology/isRecognizedCompositionOf -->

    <owl:ObjectProperty rdf:about="https://w3id.org/icon/ontology/isRecognizedCompositionOf">
        <owl:inverseOf rdf:resource="https://w3id.org/icon/ontology/recognizedComposition"/>
        <rdfs:domain rdf:resource="https://w3id.org/icon/ontology/Composition"/>
        <rdfs:range rdf:resource="https://w3id.org/icon/ontology/PreiconographicalRecognition"/>
        <rdfs:comment xml:lang="en">Inverse property of recognizedComposition</rdfs:comment>
        <rdfs:isDefinedBy rdf:resource="https://w3id.org/icon/ontology/ICONOntology"/>
        <rdfs:label xml:lang="en">Is Recognized Composition Of</rdfs:label>
    </owl:ObjectProperty>
    


    <!-- https://w3id.org/icon/ontology/isRecognizedConceptOf -->

    <owl:ObjectProperty rdf:about="https://w3id.org/icon/ontology/isRecognizedConceptOf">
        <owl:inverseOf rdf:resource="https://w3id.org/icon/ontology/recognizedConcept"/>
        <rdfs:domain rdf:resource="http://www.ontologydesignpatterns.org/ont/dul/DUL.owl#SocialObject"/>
        <rdfs:range rdf:resource="https://w3id.org/icon/ontology/IntrinsicMeaning"/>
        <rdfs:comment xml:lang="en">Inverse property of recognizedConcept</rdfs:comment>
        <rdfs:isDefinedBy rdf:resource="https://w3id.org/icon/ontology/ICONOntology"/>
        <rdfs:label xml:lang="en">Is Recognized Concept Of</rdfs:label>
    </owl:ObjectProperty>
    


    <!-- https://w3id.org/icon/ontology/isSymbolOf -->

    <owl:ObjectProperty rdf:about="https://w3id.org/icon/ontology/isSymbolOf">
        <rdfs:domain>
            <owl:Class>
                <owl:unionOf rdf:parseType="Collection">
                    <rdf:Description rdf:about="https://w3id.org/icon/ontology/Symbol"/>
                    <rdf:Description rdf:about="https://www.w3id.org/simulation/ontology/Simulation"/>
                </owl:unionOf>
            </owl:Class>
        </rdfs:domain>
        <rdfs:range rdf:resource="https://w3id.org/icon/ontology/Image"/>
        <rdfs:comment xml:lang="en">Inverse property of has symbol</rdfs:comment>
        <rdfs:isDefinedBy rdf:resource="https://w3id.org/icon/ontology/ICONOntology"/>
        <rdfs:label xml:lang="en">Is Symbol Of</rdfs:label>
    </owl:ObjectProperty>
    


    <!-- https://w3id.org/icon/ontology/partOf -->

    <owl:ObjectProperty rdf:about="https://w3id.org/icon/ontology/partOf">
        <rdfs:subPropertyOf rdf:resource="http://www.ontologydesignpatterns.org/ont/dul/DUL.owl#isPartOf"/>
        <rdfs:domain rdf:resource="https://w3id.org/icon/ontology/ArtisticMotif"/>
        <rdfs:range rdf:resource="https://w3id.org/icon/ontology/Composition"/>
        <rdfs:comment xml:lang="en">Inverse property of hasPart</rdfs:comment>
        <rdfs:label xml:lang="en">Part Of (ICON)</rdfs:label>
    </owl:ObjectProperty>
    


    <!-- https://w3id.org/icon/ontology/preiconographicallyCompliesWith -->

    <owl:ObjectProperty rdf:about="https://w3id.org/icon/ontology/preiconographicallyCompliesWith">
        <rdfs:subPropertyOf rdf:resource="http://www.ontologydesignpatterns.org/ont/dul/DUL.owl#satisfies"/>
        <rdfs:domain>
            <owl:Class>
                <owl:unionOf rdf:parseType="Collection">
                    <rdf:Description rdf:about="https://w3id.org/icon/ontology/FormalMotifRecognition"/>
                    <rdf:Description rdf:about="https://w3id.org/icon/ontology/PreiconographicalRecognition"/>
                </owl:unionOf>
            </owl:Class>
        </rdfs:domain>
        <rdfs:range rdf:resource="https://w3id.org/icon/ontology/InterpretationDescription"/>
        <rdfs:comment xml:lang="en">This property is used to link all the pre-iconographical and formal motif recognitions recognitions that take part in one or more interpretation(s), to that/those interpretation(s)</rdfs:comment>
        <rdfs:isDefinedBy rdf:resource="https://w3id.org/icon/ontology/ICONOntology"/>
        <rdfs:label xml:lang="en">pre-iconographically complies with</rdfs:label>
    </owl:ObjectProperty>
    


    <!-- https://w3id.org/icon/ontology/recognizedArtisticMotif -->

    <owl:ObjectProperty rdf:about="https://w3id.org/icon/ontology/recognizedArtisticMotif">
        <rdfs:domain rdf:resource="https://w3id.org/icon/ontology/PreiconographicalRecognition"/>
        <rdfs:range rdf:resource="https://w3id.org/icon/ontology/ArtisticMotif"/>
        <skos:broadMatch rdf:resource="http://erlangen-crm.org/current/P141_assigned"/>
    </owl:ObjectProperty>
    


    <!-- https://w3id.org/icon/ontology/recognizedComposition -->

    <owl:ObjectProperty rdf:about="https://w3id.org/icon/ontology/recognizedComposition">
        <rdfs:domain rdf:resource="https://w3id.org/icon/ontology/PreiconographicalRecognition"/>
        <rdfs:range rdf:resource="https://w3id.org/icon/ontology/Composition"/>
        <skos:broadMatch rdf:resource="http://erlangen-crm.org/current/P141_assigned"/>
    </owl:ObjectProperty>
    


    <!-- https://w3id.org/icon/ontology/recognizedConcept -->

    <owl:ObjectProperty rdf:about="https://w3id.org/icon/ontology/recognizedConcept">
        <rdfs:domain rdf:resource="https://w3id.org/icon/ontology/IntrinsicMeaning"/>
        <rdfs:range rdf:resource="http://www.ontologydesignpatterns.org/ont/dul/DUL.owl#SocialObject"/>
        <rdfs:comment xml:lang="en">This relation expresses the Concept that is related to the Intrinsic Meaning</rdfs:comment>
        <rdfs:isDefinedBy rdf:resource="https://w3id.org/icon/ontology/ICONOntology"/>
        <rdfs:label xml:lang="en">Recognized Concept</rdfs:label>
    </owl:ObjectProperty>
    


    <!-- https://w3id.org/icon/ontology/recognizedCulturalPhenomenon -->

    <owl:ObjectProperty rdf:about="https://w3id.org/icon/ontology/recognizedCulturalPhenomenon">
        <rdfs:domain rdf:resource="https://w3id.org/icon/ontology/IntrinsicMeaning"/>
        <rdfs:range rdf:resource="https://w3id.org/icon/ontology/CulturalPhenomenon"/>
        <rdfs:comment xml:lang="en">This relation expresses the Cultural Phenomenon that is related to the Intrinsic Meaning</rdfs:comment>
        <rdfs:isDefinedBy rdf:resource="https://w3id.org/icon/ontology/ICONOntology"/>
        <rdfs:label xml:lang="en">Recognized Cultural Phenomenon</rdfs:label>
    </owl:ObjectProperty>
    


    <!-- https://w3id.org/icon/ontology/recognizedGenre -->

    <owl:ObjectProperty rdf:about="https://w3id.org/icon/ontology/recognizedGenre">
        <rdfs:subPropertyOf rdf:resource="http://erlangen-crm.org/current/P141_assigned"/>
        <rdfs:domain rdf:resource="https://w3id.org/icon/ontology/Recognition"/>
        <rdfs:range rdf:resource="https://w3id.org/icon/ontology/ArtGenre"/>
        <rdfs:comment xml:lang="en">This property is substituted by the the solution adopted by linked.art using crm:P2_has_type as follows: &lt;subject&gt;, crm:P2_has_type, &lt;specific style term&gt;.  &lt;specific style term&gt; crm:P2_has_type, &lt;http://vocab.getty.edu/aat/300015646&gt; # the AAT term indicating the concept of style.</rdfs:comment>
        <rdfs:label xml:lang="en">Recognized Genre</rdfs:label>
        <owl:deprecated xml:lang="en">since new version 25/03</owl:deprecated>
    </owl:ObjectProperty>
    


    <!-- https://w3id.org/icon/ontology/recognizedImage -->

    <owl:ObjectProperty rdf:about="https://w3id.org/icon/ontology/recognizedImage">
        <rdfs:domain rdf:resource="https://w3id.org/icon/ontology/IconographicalRecognition"/>
        <rdfs:range rdf:resource="https://w3id.org/icon/ontology/Image"/>
        <skos:broadMatch rdf:resource="http://erlangen-crm.org/current/P141_assigned"/>
    </owl:ObjectProperty>
    


    <!-- https://w3id.org/icon/ontology/recognizedIntrinsicMeaning -->

    <owl:ObjectProperty rdf:about="https://w3id.org/icon/ontology/recognizedIntrinsicMeaning">
        <rdfs:subPropertyOf rdf:resource="http://www.w3.org/2002/07/owl#topObjectProperty"/>
        <rdfs:domain rdf:resource="https://w3id.org/icon/ontology/IconologicalRecognition"/>
        <rdfs:range rdf:resource="https://w3id.org/icon/ontology/IntrinsicMeaning"/>
        <rdfs:comment xml:lang="en">This relation associates the Intrinsic Meaning to the Iconological Recognition that recognizes it at the third level of interpretation.</rdfs:comment>
        <rdfs:isDefinedBy rdf:resource="https://w3id.org/icon/ontology/ICONOntology"/>
        <rdfs:label xml:lang="en">Recognized Intrinsic Meaning</rdfs:label>
    </owl:ObjectProperty>
    


    <!-- https://w3id.org/icon/ontology/recognizedInvenzione -->

    <owl:ObjectProperty rdf:about="https://w3id.org/icon/ontology/recognizedInvenzione">
        <rdfs:domain rdf:resource="https://w3id.org/icon/ontology/IconographicalRecognition"/>
        <rdfs:range rdf:resource="https://w3id.org/icon/ontology/Invenzione"/>
        <skos:broadMatch rdf:resource="http://erlangen-crm.org/current/P141_assigned"/>
    </owl:ObjectProperty>
    


    <!-- https://w3id.org/icon/ontology/refersToArtisticMotif -->

    <owl:ObjectProperty rdf:about="https://w3id.org/icon/ontology/refersToArtisticMotif">
        <rdfs:subPropertyOf rdf:resource="http://erlangen-crm.org/current/P140_assigned_attribute_to"/>
        <rdfs:domain rdf:resource="https://w3id.org/icon/ontology/IconographicalRecognition"/>
        <rdfs:range>
            <owl:Class>
                <owl:unionOf rdf:parseType="Collection">
                    <rdf:Description rdf:about="https://w3id.org/icon/ontology/ArtisticMotif"/>
                    <rdf:Description rdf:about="https://w3id.org/icon/ontology/Composition"/>
                </owl:unionOf>
            </owl:Class>
        </rdfs:range>
        <rdfs:comment xml:lang="en">This relation associates a Composition or an Artistic Motif to the Iconographical Recognition that describes it at the second level of interpretation.</rdfs:comment>
        <rdfs:label xml:lang="en">Refers To Artistic Motif</rdfs:label>
    </owl:ObjectProperty>
    


    <!-- https://w3id.org/icon/ontology/takesPartIn -->

    <owl:ObjectProperty rdf:about="https://w3id.org/icon/ontology/takesPartIn">
        <rdfs:domain>
            <owl:Class>
                <owl:unionOf rdf:parseType="Collection">
                    <rdf:Description rdf:about="https://w3id.org/icon/ontology/Character"/>
                    <rdf:Description rdf:about="https://w3id.org/icon/ontology/Event"/>
                    <rdf:Description rdf:about="https://w3id.org/icon/ontology/NamedObject"/>
                    <rdf:Description rdf:about="https://w3id.org/icon/ontology/Personification"/>
                    <rdf:Description rdf:about="https://w3id.org/icon/ontology/Place"/>
                    <rdf:Description rdf:about="https://w3id.org/icon/ontology/Symbol"/>
                </owl:unionOf>
            </owl:Class>
        </rdfs:domain>
        <rdfs:range rdf:resource="https://w3id.org/icon/ontology/Invenzione"/>
        <rdfs:comment xml:lang="en">Inverse property of composed of</rdfs:comment>
        <rdfs:isDefinedBy rdf:resource="https://w3id.org/icon/ontology/ICONOntology"/>
        <rdfs:label xml:lang="en">Takes part in</rdfs:label>
    </owl:ObjectProperty>
    


    <!-- 
    ///////////////////////////////////////////////////////////////////////////////////////
    //
    // Data properties
    //
    ///////////////////////////////////////////////////////////////////////////////////////
     -->

    


    <!-- https://w3id.org/icon/ontology/regionDescription -->

    <owl:DatatypeProperty rdf:about="https://w3id.org/icon/ontology/regionDescription">
        <rdfs:domain>
            <owl:Class>
                <owl:unionOf rdf:parseType="Collection">
                    <rdf:Description rdf:about="https://w3id.org/icon/ontology/ArtisticMotif"/>
                    <rdf:Description rdf:about="https://w3id.org/icon/ontology/Composition"/>
                </owl:unionOf>
            </owl:Class>
        </rdfs:domain>
        <rdfs:range rdf:resource="http://www.w3.org/2000/01/rdf-schema#Literal"/>
    </owl:DatatypeProperty>
    


    <!-- 
    ///////////////////////////////////////////////////////////////////////////////////////
    //
    // Classes
    //
    ///////////////////////////////////////////////////////////////////////////////////////
     -->

    


    <!-- http://iflastandards.info/ns/fr/frbr/frbroo/F38 -->

    <owl:Class rdf:about="http://iflastandards.info/ns/fr/frbr/frbroo/F38">
        <rdfs:subClassOf rdf:resource="http://erlangen-crm.org/current/E28_Conceptual_Object"/>
    </owl:Class>
    


    <!-- http://purl.org/emmedi/hico/InterpretationAct -->

    <owl:Class rdf:about="http://purl.org/emmedi/hico/InterpretationAct"/>
    


    <!-- http://w3id.org/vir#IC11_Personification -->

    <owl:Class rdf:about="http://w3id.org/vir#IC11_Personification"/>
    


    <!-- http://w3id.org/vir#IC1_Iconographical_Atom -->

    <owl:Class rdf:about="http://w3id.org/vir#IC1_Iconographical_Atom"/>
    


    <!-- http://www.ontologydesignpatterns.org/ont/dul/DUL.owl#SocialObject -->

    <rdf:Description rdf:about="http://www.ontologydesignpatterns.org/ont/dul/DUL.owl#SocialObject">
        <rdfs:subClassOf rdf:resource="https://w3id.org/arco/ontology/context-description/Subject"/>
    </rdf:Description>
    


    <!-- https://w3id.org/arco/ontology/arco/HistoricOrArtisticProperty -->

    <owl:Class rdf:about="https://w3id.org/arco/ontology/arco/HistoricOrArtisticProperty"/>
    


    <!-- https://w3id.org/arco/ontology/context-description/Subject -->

    <owl:Class rdf:about="https://w3id.org/arco/ontology/context-description/Subject">
        <owl:disjointWith rdf:resource="https://w3id.org/icon/ontology/VisualSubject"/>
    </owl:Class>
    


    <!-- https://w3id.org/icon/ontology/Action -->

    <owl:Class rdf:about="https://w3id.org/icon/ontology/Action">
        <rdfs:subClassOf rdf:resource="http://www.ontologydesignpatterns.org/ont/dul/DUL.owl#Event"/>
        <rdfs:subClassOf rdf:resource="https://w3id.org/arco/ontology/context-description/Subject"/>
        <skos:broadMatch rdf:resource="http://erlangen-crm.org/current/E5_Event"/>
    </owl:Class>
    


    <!-- https://w3id.org/icon/ontology/Allegory -->

    <owl:Class rdf:about="https://w3id.org/icon/ontology/Allegory">
        <rdfs:subClassOf rdf:resource="https://w3id.org/icon/ontology/Invenzione"/>
        <rdfs:subClassOf>
            <owl:Class>
                <owl:unionOf rdf:parseType="Collection">
                    <owl:Restriction>
                        <owl:onProperty rdf:resource="https://w3id.org/icon/ontology/composedOf"/>
                        <owl:someValuesFrom rdf:resource="https://w3id.org/icon/ontology/Personification"/>
                    </owl:Restriction>
                    <owl:Restriction>
                        <owl:onProperty rdf:resource="https://w3id.org/icon/ontology/composedOf"/>
                        <owl:someValuesFrom rdf:resource="https://w3id.org/icon/ontology/Symbol"/>
                    </owl:Restriction>
                </owl:unionOf>
            </owl:Class>
        </rdfs:subClassOf>
        <skos:broadMatch rdf:resource="http://erlangen-crm.org/current/E1_CRM_Entity"/>
    </owl:Class>
    


    <!-- https://w3id.org/icon/ontology/ArtGenre -->

    <owl:Class rdf:about="https://w3id.org/icon/ontology/ArtGenre">
        <rdfs:comment xml:lang="en">This class is substituted by the the solution adopted by linked.art using crm:P2_has_type as follows: &lt;subject&gt;, crm:P2_has_type, &lt;specific style term&gt;.  &lt;specific style term&gt; crm:P2_has_type, &lt;http://vocab.getty.edu/aat/300015646&gt; # the AAT term indicating the concept of style.</rdfs:comment>
        <rdfs:label xml:lang="en">Art Genre</rdfs:label>
        <owl:deprecated>since new version 25/03</owl:deprecated>
    </owl:Class>
    


    <!-- https://w3id.org/icon/ontology/ArtisticMotif -->

    <owl:Class rdf:about="https://w3id.org/icon/ontology/ArtisticMotif">
        <rdfs:subClassOf rdf:resource="https://w3id.org/icon/ontology/VisualSubject"/>
        <rdfs:subClassOf>
            <owl:Class>
                <owl:unionOf rdf:parseType="Collection">
                    <owl:Restriction>
                        <owl:onProperty rdf:resource="https://w3id.org/icon/ontology/hasExpressionalMeaning"/>
                        <owl:minQualifiedCardinality rdf:datatype="http://www.w3.org/2001/XMLSchema#nonNegativeInteger">1</owl:minQualifiedCardinality>
                        <owl:onClass rdf:resource="https://w3id.org/icon/ontology/ExpressionalQuality"/>
                    </owl:Restriction>
                    <owl:Restriction>
                        <owl:onProperty rdf:resource="https://w3id.org/icon/ontology/hasFactualMeaning"/>
                        <owl:minQualifiedCardinality rdf:datatype="http://www.w3.org/2001/XMLSchema#nonNegativeInteger">1</owl:minQualifiedCardinality>
                        <owl:onClass>
                            <owl:Class>
                                <owl:unionOf rdf:parseType="Collection">
                                    <rdf:Description rdf:about="https://w3id.org/icon/ontology/Action"/>
                                    <rdf:Description rdf:about="https://w3id.org/icon/ontology/NaturalElement"/>
                                </owl:unionOf>
                            </owl:Class>
                        </owl:onClass>
                    </owl:Restriction>
                </owl:unionOf>
            </owl:Class>
        </rdfs:subClassOf>
        <rdfs:subClassOf>
            <owl:Restriction>
                <owl:onProperty rdf:resource="https://w3id.org/icon/ontology/isRecognizedArtisticMotifOf"/>
                <owl:qualifiedCardinality rdf:datatype="http://www.w3.org/2001/XMLSchema#nonNegativeInteger">1</owl:qualifiedCardinality>
                <owl:onClass rdf:resource="https://w3id.org/icon/ontology/PreiconographicalRecognition"/>
            </owl:Restriction>
        </rdfs:subClassOf>
        <skos:broadMatch rdf:resource="http://erlangen-crm.org/current/E36_Visual_Item"/>
    </owl:Class>
    


    <!-- https://w3id.org/icon/ontology/Artwork -->

    <owl:Class rdf:about="https://w3id.org/icon/ontology/Artwork">
        <rdfs:subClassOf rdf:resource="http://www.ontologydesignpatterns.org/ont/dul/DUL.owl#InformationObject"/>
    <skos:broadMatch rdf:resource="http://erlangen-crm.org/current/E36_Visual_Item"/>
    </owl:Class>
    


    <!-- https://w3id.org/icon/ontology/Attitude -->

    <owl:Class rdf:about="https://w3id.org/icon/ontology/Attitude">
        <rdfs:subClassOf rdf:resource="https://w3id.org/icon/ontology/CulturalPhenomenon"/>
        <rdfs:comment xml:lang="en">Example term taken from Panofsky&apos;s studies, can be used as a specification of a cultural phenomemon if it can be considered an Attitude</rdfs:comment>
        <rdfs:isDefinedBy rdf:resource="https://w3id.org/icon/ontology/ICONOntology"/>
        <rdfs:label xml:lang="en">Attitude</rdfs:label>
    </owl:Class>
    


    <!-- https://w3id.org/icon/ontology/Belief -->

    <owl:Class rdf:about="https://w3id.org/icon/ontology/Belief">
        <rdfs:subClassOf rdf:resource="https://w3id.org/icon/ontology/CulturalPhenomenon"/>
        <rdfs:comment xml:lang="en">Example term taken from Panofsky&apos;s studies, can be used as a specification of a cultural phenomemon if it can be considered a Belief</rdfs:comment>
        <rdfs:isDefinedBy rdf:resource="https://w3id.org/icon/ontology/ICONOntology"/>
        <rdfs:label xml:lang="en">Belief</rdfs:label>
    </owl:Class>
    


    <!-- https://w3id.org/icon/ontology/Character -->

    <owl:Class rdf:about="https://w3id.org/icon/ontology/Character">
        <rdfs:subClassOf rdf:resource="https://w3id.org/arco/ontology/context-description/Subject"/>
    <skos:closeMatch rdf:resource="http://iflastandards.info/ns/fr/frbr/frbroo/F38"/>
    </owl:Class>
    


    <!-- https://w3id.org/icon/ontology/Composition -->

    <owl:Class rdf:about="https://w3id.org/icon/ontology/Composition">
        <rdfs:subClassOf rdf:resource="https://w3id.org/icon/ontology/VisualSubject"/>
        <rdfs:subClassOf>
            <owl:Restriction>
                <owl:onProperty rdf:resource="http://www.ontologydesignpatterns.org/ont/dul/DUL.owl#hasPart"/>
                <owl:minQualifiedCardinality rdf:datatype="http://www.w3.org/2001/XMLSchema#nonNegativeInteger">1</owl:minQualifiedCardinality>
                <owl:onClass rdf:resource="https://w3id.org/icon/ontology/ArtisticMotif"/>
            </owl:Restriction>
        </rdfs:subClassOf>
        <rdfs:subClassOf>
            <owl:Restriction>
                <owl:onProperty rdf:resource="https://w3id.org/icon/ontology/isRecognizedCompositionOf"/>
                <owl:qualifiedCardinality rdf:datatype="http://www.w3.org/2001/XMLSchema#nonNegativeInteger">1</owl:qualifiedCardinality>
                <owl:onClass rdf:resource="https://w3id.org/icon/ontology/PreiconographicalRecognition"/>
            </owl:Restriction>
        </rdfs:subClassOf>
        <skos:broadMatch rdf:resource="http://erlangen-crm.org/current/E36_Visual_Item"/>
    </owl:Class>
    


    <!-- https://w3id.org/icon/ontology/CompositionalStructure -->

    <owl:Class rdf:about="https://w3id.org/icon/ontology/CompositionalStructure">
        <rdfs:comment xml:lang="en">The compositional structure identifies relevant structures that can be recognized in the layout of Artistic Motifs in a Composition, e.g. pyramidal, symmetrical.</rdfs:comment>
        <rdfs:isDefinedBy rdf:resource="https://w3id.org/icon/ontology/ICONOntology"/>
        <rdfs:label xml:lang="en">Compositional Structure</rdfs:label>
    </owl:Class>
    


    <!-- https://w3id.org/icon/ontology/CulturalPhenomenon -->

    <owl:Class rdf:about="https://w3id.org/icon/ontology/CulturalPhenomenon">
        <rdfs:subClassOf rdf:resource="https://w3id.org/arco/ontology/context-description/Subject"/>
        <rdfs:comment xml:lang="en">The cultural phenomenon entity expresses the cultural, social and historical aspects of which the work of art can be document. The iconographical evolution of subjects can have a cultural meaning as well. Also the personal characteristics of the artist, or of the patron, can be involved (Wittkower, Van Straten). The cultural phenomena are the object of investigation of an iconological interpretation (Van Straten, 2012, p. 12), which is considered, in the current work, a level 3 interpretation.</rdfs:comment>
        <rdfs:isDefinedBy rdf:resource="https://w3id.org/icon/ontology/ICONOntology"/>
        <rdfs:label xml:lang="en">Cultural Phenomenon</rdfs:label>
    </owl:Class>
    


    <!-- https://w3id.org/icon/ontology/CulturalValue -->

    <owl:Class rdf:about="https://w3id.org/icon/ontology/CulturalValue">
        <rdfs:subClassOf rdf:resource="https://w3id.org/icon/ontology/CulturalPhenomenon"/>
        <rdfs:comment xml:lang="en">Example term taken from Panofsky&apos;s studies, can be used as a specification of a cultural phenomemon if it can be considered a CulturalValue</rdfs:comment>
        <rdfs:isDefinedBy rdf:resource="https://w3id.org/icon/ontology/ICONOntology"/>
        <rdfs:label xml:lang="en">Cultural Value</rdfs:label>
    </owl:Class>
    


    <!-- https://w3id.org/icon/ontology/Event -->

    <owl:Class rdf:about="https://w3id.org/icon/ontology/Event">
        <skos:broadMatch rdf:resource="http://erlangen-crm.org/current/E89_Propositional_Object"/>
        <rdfs:subClassOf rdf:resource="https://w3id.org/arco/ontology/context-description/Subject"/>
    </owl:Class>
    


    <!-- https://w3id.org/icon/ontology/ExpressionalQuality -->

    <owl:Class rdf:about="https://w3id.org/icon/ontology/ExpressionalQuality">
        <rdfs:subClassOf rdf:resource="http://www.ontologydesignpatterns.org/ont/dul/DUL.owl#SocialObject"/>
        <rdfs:subClassOf rdf:resource="https://w3id.org/arco/ontology/context-description/Subject"/>
        <skos:broadMatch rdf:resource="http://erlangen-crm.org/current/E1_CRM_Entity"/>
    </owl:Class>
    


    <!-- https://w3id.org/icon/ontology/FormalMotifRecognition -->

    <owl:Class rdf:about="https://w3id.org/icon/ontology/FormalMotifRecognition">
        <rdfs:subClassOf rdf:resource="https://w3id.org/icon/ontology/Recognition"/>
        <rdfs:subClassOf>
            <owl:Class>
                <owl:unionOf rdf:parseType="Collection">
                    <owl:Restriction>
                        <owl:onProperty rdf:resource="https://w3id.org/icon/ontology/hasCopiedMotif"/>
                        <owl:qualifiedCardinality rdf:datatype="http://www.w3.org/2001/XMLSchema#nonNegativeInteger">1</owl:qualifiedCardinality>
                        <owl:onClass rdf:resource="https://w3id.org/icon/ontology/ArtisticMotif"/>
                    </owl:Restriction>
                    <owl:Restriction>
                        <owl:onProperty rdf:resource="https://w3id.org/icon/ontology/hasCopiedMotif"/>
                        <owl:qualifiedCardinality rdf:datatype="http://www.w3.org/2001/XMLSchema#nonNegativeInteger">1</owl:qualifiedCardinality>
                        <owl:onClass rdf:resource="https://w3id.org/icon/ontology/Composition"/>
                    </owl:Restriction>
                </owl:unionOf>
            </owl:Class>
        </rdfs:subClassOf>
        <rdfs:subClassOf>
            <owl:Class>
                <owl:unionOf rdf:parseType="Collection">
                    <owl:Restriction>
                        <owl:onProperty rdf:resource="https://w3id.org/icon/ontology/hasPrototypicalMotif"/>
                        <owl:qualifiedCardinality rdf:datatype="http://www.w3.org/2001/XMLSchema#nonNegativeInteger">1</owl:qualifiedCardinality>
                        <owl:onClass rdf:resource="https://w3id.org/icon/ontology/ArtisticMotif"/>
                    </owl:Restriction>
                    <owl:Restriction>
                        <owl:onProperty rdf:resource="https://w3id.org/icon/ontology/hasPrototypicalMotif"/>
                        <owl:qualifiedCardinality rdf:datatype="http://www.w3.org/2001/XMLSchema#nonNegativeInteger">1</owl:qualifiedCardinality>
                        <owl:onClass rdf:resource="https://w3id.org/icon/ontology/Composition"/>
                    </owl:Restriction>
                </owl:unionOf>
            </owl:Class>
        </rdfs:subClassOf>
        <rdfs:comment xml:lang="en">The act of recognizing that subjects depicted by different artworks has the same formal motifs although the content represented may be different. The need of the usage of this class emerged from a bottom-up approach, rather than Panofsky&apos;s theory. It describes that certain subjects are prototypes of others, including preliminary drawings, but also cases in which another artist copied only the composition or gestures from another artwork. This recognition can link every specific part of a representation to the specific prototypes. The relation is between level 1 objects, i.e. Artistic Motifs and Composition, since it describes a formal aspect. Example of usage: if Hercules carrying the Boar is the prototype for a Christ carrying a deer, symbol of the human souls, it&apos;s possible to relate directly the boar represented in the former artwork to the deer represented in the latter.</rdfs:comment>
        <rdfs:label xml:lang="en">Formal Motif Recognition</rdfs:label>
    </owl:Class>
    


    <!-- https://w3id.org/icon/ontology/IconographicalDescription -->

    <owl:Class rdf:about="https://w3id.org/icon/ontology/IconographicalDescription">
        <rdfs:subClassOf rdf:resource="https://w3id.org/icon/ontology/InterpretationDescription"/>
        <rdfs:subClassOf>
            <owl:Restriction>
                <owl:onProperty rdf:resource="http://erlangen-crm.org/current/P70_documents"/>
                <owl:allValuesFrom rdf:resource="https://w3id.org/icon/ontology/IconographicalRecognition"/>
            </owl:Restriction>
        </rdfs:subClassOf>
        <rdfs:comment xml:lang="en">An Iconographical Description is the enumeration of iconographical recognitions of images or invenzioni recognized by one or more agents. It is thus a collection of triples. It is the summary of what would be called in Panofsky&apos;s term the second level of interpretation.</rdfs:comment>
        <rdfs:label xml:lang="en">Iconographical Description</rdfs:label>
        <owl:deprecated>from version 1.1</owl:deprecated>
    </owl:Class>
    


    <!-- https://w3id.org/icon/ontology/IconographicalRecognition -->

    <owl:Class rdf:about="https://w3id.org/icon/ontology/IconographicalRecognition">
        <rdfs:subClassOf rdf:resource="https://w3id.org/icon/ontology/Recognition"/>
        <rdfs:subClassOf>
            <owl:Class>
                <owl:unionOf rdf:parseType="Collection">
                    <owl:Restriction>
                        <owl:onProperty rdf:resource="https://w3id.org/icon/ontology/recognizedImage"/>
                        <owl:qualifiedCardinality rdf:datatype="http://www.w3.org/2001/XMLSchema#nonNegativeInteger">1</owl:qualifiedCardinality>
                        <owl:onClass rdf:resource="https://w3id.org/icon/ontology/Image"/>
                    </owl:Restriction>
                    <owl:Restriction>
                        <owl:onProperty rdf:resource="https://w3id.org/icon/ontology/recognizedInvenzione"/>
                        <owl:qualifiedCardinality rdf:datatype="http://www.w3.org/2001/XMLSchema#nonNegativeInteger">1</owl:qualifiedCardinality>
                        <owl:onClass rdf:resource="https://w3id.org/icon/ontology/Invenzione"/>
                    </owl:Restriction>
                </owl:unionOf>
            </owl:Class>
        </rdfs:subClassOf>
        <rdfs:comment xml:lang="en">A Iconographical Recognition is a n-ary relationship class that links the artwork described (and, if available, the Artistic Motifs recognized at the previous level along with their compositions) to the Images recognized, or directly to the Invenzione that results from the grouping of the subject depicted by each single image. The N-ary structure is necessary in order to include relevant additional information concerning the visual interpretation claimed.</rdfs:comment>
        <rdfs:label xml:lang="en">Iconographical Recognition</rdfs:label>
    </owl:Class>
    


    <!-- https://w3id.org/icon/ontology/IconographicalSynthesis -->

    <owl:Class rdf:about="https://w3id.org/icon/ontology/IconographicalSynthesis">
        <rdfs:subClassOf rdf:resource="https://w3id.org/icon/ontology/InterpretationDescription"/>
        <rdfs:subClassOf>
            <owl:Restriction>
                <owl:onProperty rdf:resource="http://erlangen-crm.org/current/P70_documents"/>
                <owl:allValuesFrom rdf:resource="https://w3id.org/icon/ontology/IconologicalRecognition"/>
            </owl:Restriction>
        </rdfs:subClassOf>
        <rdfs:comment xml:lang="en">An Iconographical Synthesis is the enumeration of iconological recognitions of intrinsic meanings recognized by one or more agents concerning a work of art. It is thus a collection of triples. It is the summary of what would be called in Panofsky&apos;s term the third level of interpretation.</rdfs:comment>
        <rdfs:label xml:lang="en">Iconographical Synthesis</rdfs:label>
        <owl:deprecated>from version 1.1</owl:deprecated>
    </owl:Class>
    


    <!-- https://w3id.org/icon/ontology/IconologicalRecognition -->

    <owl:Class rdf:about="https://w3id.org/icon/ontology/IconologicalRecognition">
        <rdfs:subClassOf rdf:resource="https://w3id.org/icon/ontology/Recognition"/>
        <rdfs:subClassOf>
            <owl:Restriction>
                <owl:onProperty rdf:resource="https://w3id.org/icon/ontology/recognizedIntrinsicMeaning"/>
                <owl:qualifiedCardinality rdf:datatype="http://www.w3.org/2001/XMLSchema#nonNegativeInteger">1</owl:qualifiedCardinality>
                <owl:onClass rdf:resource="https://w3id.org/icon/ontology/IntrinsicMeaning"/>
            </owl:Restriction>
        </rdfs:subClassOf>
        <rdfs:comment xml:lang="en">An Iconological Recognition is a n-ary relationship class that links the artwork described (and optionally all the subjects represented at the first and second level of interpretation) to the Intrinsic Meanings recognized. The N-ary structure is necessary in order to include relevant additional information concerning the visual interpretation claimed. This class can represent: (1) the third level act of Interpretation described by Panofsky (1939), without a distinction between a overall artwork symbolic meaning and a societal aspect, (2) the third and second level described by Van Straten, according to the value associated to the intrinsic meaning, (3) the iconic act of interpretation described by Imdahl (2012), when the intrinsic meaning is directly linked to level 1 characteristics of the image.</rdfs:comment>
        <rdfs:label xml:lang="en">Iconological Recognition</rdfs:label>
    </owl:Class>
    


    <!-- https://w3id.org/icon/ontology/Image -->

    <owl:Class rdf:about="https://w3id.org/icon/ontology/Image">
        <rdfs:subClassOf rdf:resource="https://w3id.org/icon/ontology/VisualSubject"/>
        <rdfs:subClassOf>
            <owl:Class>
                <owl:unionOf rdf:parseType="Collection">
                    <owl:Restriction>
                        <owl:onProperty rdf:resource="https://w3id.org/icon/ontology/hasCharacter"/>
                        <owl:minQualifiedCardinality rdf:datatype="http://www.w3.org/2001/XMLSchema#nonNegativeInteger">1</owl:minQualifiedCardinality>
                        <owl:onClass rdf:resource="https://w3id.org/icon/ontology/Character"/>
                    </owl:Restriction>
                    <owl:Restriction>
                        <owl:onProperty rdf:resource="https://w3id.org/icon/ontology/hasEvent"/>
                        <owl:minQualifiedCardinality rdf:datatype="http://www.w3.org/2001/XMLSchema#nonNegativeInteger">1</owl:minQualifiedCardinality>
                        <owl:onClass rdf:resource="https://w3id.org/icon/ontology/Event"/>
                    </owl:Restriction>
                    <owl:Restriction>
                        <owl:onProperty rdf:resource="https://w3id.org/icon/ontology/hasNamedObject"/>
                        <owl:minQualifiedCardinality rdf:datatype="http://www.w3.org/2001/XMLSchema#nonNegativeInteger">1</owl:minQualifiedCardinality>
                        <owl:onClass rdf:resource="https://w3id.org/icon/ontology/NamedObject"/>
                    </owl:Restriction>
                    <owl:Restriction>
                        <owl:onProperty rdf:resource="https://w3id.org/icon/ontology/hasPersonification"/>
                        <owl:minQualifiedCardinality rdf:datatype="http://www.w3.org/2001/XMLSchema#nonNegativeInteger">1</owl:minQualifiedCardinality>
                        <owl:onClass rdf:resource="https://w3id.org/icon/ontology/Personification"/>
                    </owl:Restriction>
                    <owl:Restriction>
                        <owl:onProperty rdf:resource="https://w3id.org/icon/ontology/hasPlace"/>
                        <owl:minQualifiedCardinality rdf:datatype="http://www.w3.org/2001/XMLSchema#nonNegativeInteger">1</owl:minQualifiedCardinality>
                        <owl:onClass rdf:resource="https://w3id.org/icon/ontology/Place"/>
                    </owl:Restriction>
                    <owl:Restriction>
                        <owl:onProperty rdf:resource="https://w3id.org/icon/ontology/hasSymbol"/>
                        <owl:minQualifiedCardinality rdf:datatype="http://www.w3.org/2001/XMLSchema#nonNegativeInteger">1</owl:minQualifiedCardinality>
                        <owl:onClass>
                            <owl:Class>
                                <owl:unionOf rdf:parseType="Collection">
                                    <rdf:Description rdf:about="https://w3id.org/icon/ontology/Symbol"/>
                                    <rdf:Description rdf:about="https://www.w3id.org/simulation/ontology/Simulation"/>
                                </owl:unionOf>
                            </owl:Class>
                        </owl:onClass>
                    </owl:Restriction>
                </owl:unionOf>
            </owl:Class>
        </rdfs:subClassOf>
        <rdfs:subClassOf>
            <owl:Restriction>
                <owl:onProperty rdf:resource="https://w3id.org/icon/ontology/isIconographicallyRecognizedBy"/>
                <owl:qualifiedCardinality rdf:datatype="http://www.w3.org/2001/XMLSchema#nonNegativeInteger">1</owl:qualifiedCardinality>
                <owl:onClass rdf:resource="https://w3id.org/icon/ontology/IconographicalRecognition"/>
            </owl:Restriction>
        </rdfs:subClassOf>
        <skos:broadMatch rdf:resource="http://erlangen-crm.org/current/E36_Visual_Item"/>
    </owl:Class>
    


    <!-- https://w3id.org/icon/ontology/InterpretationDescription -->

    <owl:Class rdf:about="https://w3id.org/icon/ontology/InterpretationDescription">
        <rdfs:subClassOf rdf:resource="http://www.ontologydesignpatterns.org/ont/dul/DUL.owl#Description"/>
        <rdfs:subClassOf>
            <owl:Restriction>
                <owl:onProperty rdf:resource="https://w3id.org/icon/ontology/isCompliantWithIconographicalRecognition"/>
                <owl:someValuesFrom rdf:resource="https://w3id.org/icon/ontology/IconographicalRecognition"/>
            </owl:Restriction>
        </rdfs:subClassOf>
        <rdfs:subClassOf>
            <owl:Restriction>
                <owl:onProperty rdf:resource="https://w3id.org/icon/ontology/isCompliantWithIconologicalRecognition"/>
                <owl:someValuesFrom rdf:resource="https://w3id.org/icon/ontology/IconologicalRecognition"/>
            </owl:Restriction>
        </rdfs:subClassOf>
        <rdfs:subClassOf>
            <owl:Restriction>
                <owl:onProperty rdf:resource="https://w3id.org/icon/ontology/isCompliantWithPreiconographicalRecognition"/>
                <owl:someValuesFrom>
                    <owl:Class>
                        <owl:unionOf rdf:parseType="Collection">
                            <rdf:Description rdf:about="https://w3id.org/icon/ontology/FormalMotifRecognition"/>
                            <rdf:Description rdf:about="https://w3id.org/icon/ontology/PreiconographicalRecognition"/>
                        </owl:unionOf>
                    </owl:Class>
                </owl:someValuesFrom>
            </owl:Restriction>
        </rdfs:subClassOf>
        <skos:narrowMatch rdf:resource="http://erlangen-crm.org/current/E31_Document"/>
    </owl:Class>
    


    <!-- https://w3id.org/icon/ontology/IntrinsicMeaning -->

    <owl:Class rdf:about="https://w3id.org/icon/ontology/IntrinsicMeaning">
        <rdfs:subClassOf rdf:resource="https://w3id.org/icon/ontology/VisualSubject"/>
        <rdfs:subClassOf>
            <owl:Class>
                <owl:unionOf rdf:parseType="Collection">
                    <owl:Class>
                        <owl:intersectionOf rdf:parseType="Collection">
                            <owl:Restriction>
                                <owl:onProperty rdf:resource="https://w3id.org/icon/ontology/recognizedConcept"/>
                                <owl:qualifiedCardinality rdf:datatype="http://www.w3.org/2001/XMLSchema#nonNegativeInteger">1</owl:qualifiedCardinality>
                                <owl:onClass rdf:resource="http://www.ontologydesignpatterns.org/ont/dul/DUL.owl#SocialObject"/>
                            </owl:Restriction>
                            <owl:Restriction>
                                <owl:onProperty rdf:resource="https://w3id.org/icon/ontology/recognizedCulturalPhenomenon"/>
                                <owl:qualifiedCardinality rdf:datatype="http://www.w3.org/2001/XMLSchema#nonNegativeInteger">1</owl:qualifiedCardinality>
                                <owl:onClass rdf:resource="https://w3id.org/icon/ontology/CulturalPhenomenon"/>
                            </owl:Restriction>
                        </owl:intersectionOf>
                    </owl:Class>
                    <owl:Class>
                        <owl:unionOf rdf:parseType="Collection">
                            <owl:Restriction>
                                <owl:onProperty rdf:resource="https://w3id.org/icon/ontology/recognizedConcept"/>
                                <owl:qualifiedCardinality rdf:datatype="http://www.w3.org/2001/XMLSchema#nonNegativeInteger">1</owl:qualifiedCardinality>
                                <owl:onClass rdf:resource="http://www.ontologydesignpatterns.org/ont/dul/DUL.owl#SocialObject"/>
                            </owl:Restriction>
                            <owl:Restriction>
                                <owl:onProperty rdf:resource="https://w3id.org/icon/ontology/recognizedCulturalPhenomenon"/>
                                <owl:qualifiedCardinality rdf:datatype="http://www.w3.org/2001/XMLSchema#nonNegativeInteger">1</owl:qualifiedCardinality>
                                <owl:onClass rdf:resource="https://w3id.org/icon/ontology/CulturalPhenomenon"/>
                            </owl:Restriction>
                        </owl:unionOf>
                    </owl:Class>
                </owl:unionOf>
            </owl:Class>
        </rdfs:subClassOf>
        <rdfs:subClassOf>
            <owl:Restriction>
                <owl:onProperty rdf:resource="https://w3id.org/icon/ontology/isIntrinsicMeaningOf"/>
                <owl:qualifiedCardinality rdf:datatype="http://www.w3.org/2001/XMLSchema#nonNegativeInteger">1</owl:qualifiedCardinality>
                <owl:onClass rdf:resource="https://w3id.org/icon/ontology/IconologicalRecognition"/>
            </owl:Restriction>
        </rdfs:subClassOf>
        <skos:broadMatch rdf:resource="http://erlangen-crm.org/current/E36_Visual_Item"/>
    </owl:Class>
    


    <!-- https://w3id.org/icon/ontology/Invenzione -->

    <owl:Class rdf:about="https://w3id.org/icon/ontology/Invenzione">
        <rdfs:subClassOf rdf:resource="https://w3id.org/arco/ontology/context-description/Subject"/>
        <skos:broadMatch rdf:resource="http://erlangen-crm.org/current/E1_CRM_Entity"/>
    </owl:Class>
    


    <!-- https://w3id.org/icon/ontology/NamedObject -->

    <owl:Class rdf:about="https://w3id.org/icon/ontology/NamedObject">
        <skos:broadMatch rdf:resource="http://erlangen-crm.org/current/E89_Propositional_Object"/>
        <rdfs:subClassOf rdf:resource="https://w3id.org/arco/ontology/context-description/Subject"/>
    </owl:Class>
    


    <!-- https://w3id.org/icon/ontology/NaturalElement -->

    <owl:Class rdf:about="https://w3id.org/icon/ontology/NaturalElement">
        <skos:broadMatch rdf:resource="http://erlangen-crm.org/current/E1_CRM_Entity"/>
        <rdfs:subClassOf rdf:resource="https://w3id.org/arco/ontology/context-description/Subject"/>
    </owl:Class>
    


    <!-- https://w3id.org/icon/ontology/Personification -->

    <owl:Class rdf:about="https://w3id.org/icon/ontology/Personification">
        <skos:closeMatch rdf:resource="http://w3id.org/vir#IC11_Personification"/>
        <rdfs:subClassOf rdf:resource="https://w3id.org/arco/ontology/context-description/Subject"/>
    </owl:Class>
    


    <!-- https://w3id.org/icon/ontology/Place -->

    <owl:Class rdf:about="https://w3id.org/icon/ontology/Place">
        <skos:broadMatch rdf:resource="http://erlangen-crm.org/current/E89_Propositional_Object"/>
        <rdfs:subClassOf rdf:resource="https://w3id.org/arco/ontology/context-description/Subject"/>
    </owl:Class>
    


    <!-- https://w3id.org/icon/ontology/PreiconographicalDescription -->

    <owl:Class rdf:about="https://w3id.org/icon/ontology/PreiconographicalDescription">
        <rdfs:subClassOf rdf:resource="https://w3id.org/icon/ontology/InterpretationDescription"/>
        <rdfs:subClassOf>
            <owl:Restriction>
                <owl:onProperty rdf:resource="http://erlangen-crm.org/current/P70_documents"/>
                <owl:allValuesFrom>
                    <owl:Class>
                        <owl:unionOf rdf:parseType="Collection">
                            <rdf:Description rdf:about="https://w3id.org/icon/ontology/FormalMotifRecognition"/>
                            <rdf:Description rdf:about="https://w3id.org/icon/ontology/PreiconographicalRecognition"/>
                        </owl:unionOf>
                    </owl:Class>
                </owl:allValuesFrom>
            </owl:Restriction>
        </rdfs:subClassOf>
        <rdfs:comment xml:lang="en">A Pre-iconographical description is the enumeration of the Pre-Iconographical Recognitions of a certain work of art, performed by one or more agents. It is thus a collection of triples constituting the documentation of the interpretation at level 1. The term and its definition is taken from Panofsky&apos;s Studies in Iconology (1939).</rdfs:comment>
        <rdfs:label xml:lang="en">Preiconographical Description</rdfs:label>
        <owl:deprecated>from version 1.1</owl:deprecated>
    </owl:Class>
    


    <!-- https://w3id.org/icon/ontology/PreiconographicalRecognition -->

    <owl:Class rdf:about="https://w3id.org/icon/ontology/PreiconographicalRecognition">
        <rdfs:subClassOf rdf:resource="https://w3id.org/icon/ontology/Recognition"/>
        <rdfs:subClassOf>
            <owl:Class>
                <owl:unionOf rdf:parseType="Collection">
                    <owl:Restriction>
                        <owl:onProperty rdf:resource="https://w3id.org/icon/ontology/recognizedArtisticMotif"/>
                        <owl:qualifiedCardinality rdf:datatype="http://www.w3.org/2001/XMLSchema#nonNegativeInteger">1</owl:qualifiedCardinality>
                        <owl:onClass rdf:resource="https://w3id.org/icon/ontology/ArtisticMotif"/>
                    </owl:Restriction>
                    <owl:Restriction>
                        <owl:onProperty rdf:resource="https://w3id.org/icon/ontology/recognizedComposition"/>
                        <owl:qualifiedCardinality rdf:datatype="http://www.w3.org/2001/XMLSchema#nonNegativeInteger">1</owl:qualifiedCardinality>
                        <owl:onClass rdf:resource="https://w3id.org/icon/ontology/Composition"/>
                    </owl:Restriction>
                </owl:unionOf>
            </owl:Class>
        </rdfs:subClassOf>
        <rdfs:comment xml:lang="en">A Pre-iconographical recognition is a n-ary relationship class that links the artwork described (and optionally the Pure Forms composing it) to the Artistic Motifs recognized as carrier of meaning at the first level of analysis. The N-ary structure is necessary in order to include relevant additional information concerning the visual interpretation claimed.</rdfs:comment>
        <rdfs:label xml:lang="en">Preiconographical Recognition</rdfs:label>
    </owl:Class>
    


    <!-- https://w3id.org/icon/ontology/PureForm -->

    <owl:Class rdf:about="https://w3id.org/icon/ontology/PureForm">
        <rdfs:comment xml:lang="en">A pure form represents the physical portion of the work of art in which artistic motifs are found. It has been introduced as a way to include the results of analysis performed by computational agents, that are able to classify images and give image coordinates for specific recognition. It is not recommended to be used by manual annotators or in any case in which the coordinates of the image of the work of art are not considered. If available, the Pure form can represent the region of an image identified by IIIF Image API.</rdfs:comment>
        <rdfs:comment>Change the definition to the formal representation that can be enclosed in a certain coordinate.</rdfs:comment>
        <rdfs:label xml:lang="en">Pure Form</rdfs:label>
        <owl:deprecated>from 1.1 version</owl:deprecated>
    </owl:Class>
    


    <!-- https://w3id.org/icon/ontology/Recognition -->

    <owl:Class rdf:about="https://w3id.org/icon/ontology/Recognition">
        <rdfs:subClassOf rdf:resource="http://purl.org/emmedi/hico/InterpretationAct"/>
        <rdfs:subClassOf rdf:resource="http://www.ontologydesignpatterns.org/ont/dul/DUL.owl#Situation"/>
        <rdfs:subClassOf>
            <owl:Restriction>
                <owl:onProperty rdf:resource="https://w3id.org/icon/ontology/aboutWorkOfArt"/>
                <owl:qualifiedCardinality rdf:datatype="http://www.w3.org/2001/XMLSchema#nonNegativeInteger">1</owl:qualifiedCardinality>
                <owl:onClass rdf:resource="https://w3id.org/icon/ontology/Artwork"/>
            </owl:Restriction>
        </rdfs:subClassOf>
        <skos:broadMatch rdf:resource="http://erlangen-crm.org/current/E13_Attribute_Assignment"/>
    </owl:Class>
    


    <!-- https://w3id.org/icon/ontology/Story -->

    <owl:Class rdf:about="https://w3id.org/icon/ontology/Story">
        <rdfs:subClassOf rdf:resource="https://w3id.org/icon/ontology/Invenzione"/>
        <rdfs:subClassOf>
            <owl:Class>
                <owl:unionOf rdf:parseType="Collection">
                    <owl:Restriction>
                        <owl:onProperty rdf:resource="https://w3id.org/icon/ontology/composedOf"/>
                        <owl:someValuesFrom rdf:resource="http://www.ontologydesignpatterns.org/ont/dul/DUL.owl#Place"/>
                    </owl:Restriction>
                    <owl:Restriction>
                        <owl:onProperty rdf:resource="https://w3id.org/icon/ontology/composedOf"/>
                        <owl:someValuesFrom rdf:resource="https://w3id.org/icon/ontology/Character"/>
                    </owl:Restriction>
                    <owl:Restriction>
                        <owl:onProperty rdf:resource="https://w3id.org/icon/ontology/composedOf"/>
                        <owl:someValuesFrom rdf:resource="https://w3id.org/icon/ontology/Event"/>
                    </owl:Restriction>
                    <owl:Restriction>
                        <owl:onProperty rdf:resource="https://w3id.org/icon/ontology/composedOf"/>
                        <owl:someValuesFrom rdf:resource="https://w3id.org/icon/ontology/NamedObject"/>
                    </owl:Restriction>
                </owl:unionOf>
            </owl:Class>
        </rdfs:subClassOf>
        <skos:broadMatch rdf:resource="http://erlangen-crm.org/current/E1_CRM_Entity"/>
    </owl:Class>
    


    <!-- https://w3id.org/icon/ontology/Symbol -->

    <owl:Class rdf:about="https://w3id.org/icon/ontology/Symbol">
        <owl:equivalentClass rdf:resource="https://www.w3id.org/simulation/ontology/Simulation"/>
        <rdfs:subClassOf rdf:resource="https://w3id.org/arco/ontology/context-description/Subject"/>
        <skos:broadMatch rdf:resource="http://erlangen-crm.org/current/E90_Symbolic_Object"/>
    </owl:Class>
    


    <!-- https://w3id.org/icon/ontology/Tendency -->

    <owl:Class rdf:about="https://w3id.org/icon/ontology/Tendency">
        <rdfs:subClassOf rdf:resource="https://w3id.org/icon/ontology/CulturalPhenomenon"/>
        <rdfs:comment xml:lang="en">Example term taken from Panofsky&apos;s studies, can be used as a specification of a cultural phenomemon if it can be considered a tendency</rdfs:comment>
        <rdfs:isDefinedBy rdf:resource="https://w3id.org/icon/ontology/ICONOntology"/>
        <rdfs:label xml:lang="en">Tendency</rdfs:label>
    </owl:Class>
    


    <!-- https://w3id.org/icon/ontology/VisualSubject -->

    <owl:Class rdf:about="https://w3id.org/icon/ontology/VisualSubject">
        <rdfs:comment xml:lang="en">A visual subject is the representation of the subject in specific artwork, in contrast with the arco:Subject which is used to define a general subject which can be shared by multiple artworks. For example, the image representing Christ in the Last Supper is a visual Subject because it is intended as only that representation for that specific artwork. The character referred by that image (Christ) would be an arco:Subject, and it can shared by all the artworks that have a specific image that refers to Christ.</rdfs:comment>
        <rdfs:isDefinedBy rdf:resource="https://w3id.org/icon/ontology/ICONOntology"/>
        <rdfs:label xml:lang="en">Visual Subject</rdfs:label>
    </owl:Class>
    


    <!-- https://www.w3id.org/simulation/ontology/Simulation -->

    <rdf:Description rdf:about="https://www.w3id.org/simulation/ontology/Simulation"/>
    


    <!-- 
    ///////////////////////////////////////////////////////////////////////////////////////
    //
    // Individuals
    //
    ///////////////////////////////////////////////////////////////////////////////////////
     -->

    


    <!-- http://erlangen-crm.org/current/E1_CRM_Entity -->

    <owl:NamedIndividual rdf:about="http://erlangen-crm.org/current/E1_CRM_Entity"/>
    


    <!-- http://erlangen-crm.org/current/E31_Document -->

    <owl:NamedIndividual rdf:about="http://erlangen-crm.org/current/E31_Document"/>
    


    <!-- http://erlangen-crm.org/current/E5_Event -->

    <owl:NamedIndividual rdf:about="http://erlangen-crm.org/current/E5_Event"/>
    


    <!-- http://erlangen-crm.org/current/E89_Propositional_Object -->

    <owl:NamedIndividual rdf:about="http://erlangen-crm.org/current/E89_Propositional_Object"/>
    


    <!-- http://iflastandards.info/ns/fr/frbr/frbroo/F38 -->

    <owl:NamedIndividual rdf:about="http://iflastandards.info/ns/fr/frbr/frbroo/F38"/>
    


    <!-- http://w3id.org/vir#IC11_Personification -->

    <owl:NamedIndividual rdf:about="http://w3id.org/vir#IC11_Personification"/>
    


    <!-- http://w3id.org/vir#K4_is_visual_prototype_of -->

    <owl:NamedIndividual rdf:about="http://w3id.org/vir#K4_is_visual_prototype_of"/>
    


    <!-- https://w3id.org/icon/ontology/Action -->

    <owl:NamedIndividual rdf:about="https://w3id.org/icon/ontology/Action">
        <skos:broadMatch rdf:resource="http://erlangen-crm.org/current/E5_Event"/>
    </owl:NamedIndividual>
    


    <!-- https://w3id.org/icon/ontology/Allegory -->

    <owl:NamedIndividual rdf:about="https://w3id.org/icon/ontology/Allegory">
        <skos:broadMatch rdf:resource="http://erlangen-crm.org/current/E1_CRM_Entity"/>
    </owl:NamedIndividual>
    


    <!-- https://w3id.org/icon/ontology/ArtisticMotif -->

    <owl:NamedIndividual rdf:about="https://w3id.org/icon/ontology/ArtisticMotif">
        <skos:broadMatch rdf:resource="http://erlangen-crm.org/current/E36_Visual_Item"/>
    </owl:NamedIndividual>
    


    <!-- https://w3id.org/icon/ontology/Artwork -->

    <owl:NamedIndividual rdf:about="https://w3id.org/icon/ontology/Artwork">
        <skos:broadMatch rdf:resource="http://erlangen-crm.org/current/E36_Visual_Item"/>
    </owl:NamedIndividual>
    


    <!-- https://w3id.org/icon/ontology/Character -->

    <owl:NamedIndividual rdf:about="https://w3id.org/icon/ontology/Character">
        <skos:narrowMatch rdf:resource="http://iflastandards.info/ns/fr/frbr/frbroo/F38"/>
    </owl:NamedIndividual>
    


    <!-- https://w3id.org/icon/ontology/Composition -->

    <owl:NamedIndividual rdf:about="https://w3id.org/icon/ontology/Composition">
        <skos:broadMatch rdf:resource="http://erlangen-crm.org/current/E36_Visual_Item"/>
    </owl:NamedIndividual>
    


    <!-- https://w3id.org/icon/ontology/Event -->

    <owl:NamedIndividual rdf:about="https://w3id.org/icon/ontology/Event">
        <skos:broadMatch rdf:resource="http://erlangen-crm.org/current/E89_Propositional_Object"/>
    </owl:NamedIndividual>
    


    <!-- https://w3id.org/icon/ontology/ExpressionalQuality -->

    <owl:NamedIndividual rdf:about="https://w3id.org/icon/ontology/ExpressionalQuality">
        <skos:broadMatch rdf:resource="http://erlangen-crm.org/current/E1_CRM_Entity"/>
    </owl:NamedIndividual>
    


    <!-- https://w3id.org/icon/ontology/ICONOntology -->

    <owl:NamedIndividual rdf:about="https://w3id.org/icon/ontology/ICONOntology"/>
    


    <!-- https://w3id.org/icon/ontology/Image -->

    <owl:NamedIndividual rdf:about="https://w3id.org/icon/ontology/Image">
        <skos:broadMatch rdf:resource="http://erlangen-crm.org/current/E36_Visual_Item"/>
    </owl:NamedIndividual>
    


    <!-- https://w3id.org/icon/ontology/InterpretationDescription -->

    <owl:NamedIndividual rdf:about="https://w3id.org/icon/ontology/InterpretationDescription">
        <skos:narrowMatch rdf:resource="http://erlangen-crm.org/current/E31_Document"/>
    </owl:NamedIndividual>
    


    <!-- https://w3id.org/icon/ontology/IntrinsicMeaning -->

    <owl:NamedIndividual rdf:about="https://w3id.org/icon/ontology/IntrinsicMeaning">
        <skos:broadMatch rdf:resource="http://erlangen-crm.org/current/E36_Visual_Item"/>
    </owl:NamedIndividual>
    


    <!-- https://w3id.org/icon/ontology/Invenzione -->

    <owl:NamedIndividual rdf:about="https://w3id.org/icon/ontology/Invenzione">
        <skos:broadMatch rdf:resource="http://erlangen-crm.org/current/E1_CRM_Entity"/>
    </owl:NamedIndividual>
    


    <!-- https://w3id.org/icon/ontology/NamedObject -->

    <owl:NamedIndividual rdf:about="https://w3id.org/icon/ontology/NamedObject">
        <skos:broadMatch rdf:resource="http://erlangen-crm.org/current/E89_Propositional_Object"/>
    </owl:NamedIndividual>
    


    <!-- https://w3id.org/icon/ontology/NaturalElement -->

    <owl:NamedIndividual rdf:about="https://w3id.org/icon/ontology/NaturalElement">
        <skos:broadMatch rdf:resource="http://erlangen-crm.org/current/E1_CRM_Entity"/>
    </owl:NamedIndividual>
    


    <!-- https://w3id.org/icon/ontology/Personification -->

    <owl:NamedIndividual rdf:about="https://w3id.org/icon/ontology/Personification">
        <skos:closeMatch rdf:resource="http://w3id.org/vir#IC11_Personification"/>
    </owl:NamedIndividual>
    


    <!-- https://w3id.org/icon/ontology/Place -->

    <owl:NamedIndividual rdf:about="https://w3id.org/icon/ontology/Place">
        <skos:broadMatch rdf:resource="http://erlangen-crm.org/current/E89_Propositional_Object"/>
    </owl:NamedIndividual>
    


    <!-- https://w3id.org/icon/ontology/Recognition -->

    <owl:NamedIndividual rdf:about="https://w3id.org/icon/ontology/Recognition">
        <skos:broadMatch rdf:resource="http://erlangen-crm.org/current/E13_Attribute_Assignment"/>
    </owl:NamedIndividual>
    


    <!-- https://w3id.org/icon/ontology/Story -->

    <owl:NamedIndividual rdf:about="https://w3id.org/icon/ontology/Story">
        <skos:broadMatch rdf:resource="http://erlangen-crm.org/current/E1_CRM_Entity"/>
    </owl:NamedIndividual>
    


    <!-- https://w3id.org/icon/ontology/Symbol -->

    <owl:NamedIndividual rdf:about="https://w3id.org/icon/ontology/Symbol">
        <skos:broadMatch rdf:resource="http://erlangen-crm.org/current/E90_Symbolic_Object"/>
    </owl:NamedIndividual>
    


    <!-- https://w3id.org/icon/ontology/hasCharacter -->

    <owl:NamedIndividual rdf:about="https://w3id.org/icon/ontology/hasCharacter">
        <skos:broadMatch rdf:resource="http://erlangen-crm.org/current/P138_represents"/>
    </owl:NamedIndividual>
    


    <!-- https://w3id.org/icon/ontology/hasCopiedMotif -->

    <owl:NamedIndividual rdf:about="https://w3id.org/icon/ontology/hasCopiedMotif">
        <skos:broadMatch rdf:resource="http://w3id.org/vir#K4_is_visual_prototype_of"/>
    </owl:NamedIndividual>
    


    <!-- https://w3id.org/icon/ontology/hasEvent -->

    <owl:NamedIndividual rdf:about="https://w3id.org/icon/ontology/hasEvent">
        <skos:broadMatch rdf:resource="http://erlangen-crm.org/current/P138_represents"/>
    </owl:NamedIndividual>
    


    <!-- https://w3id.org/icon/ontology/hasExpressionalMeaning -->

    <owl:NamedIndividual rdf:about="https://w3id.org/icon/ontology/hasExpressionalMeaning">
        <skos:broadMatch rdf:resource="http://erlangen-crm.org/current/P138_represents"/>
    </owl:NamedIndividual>
    


    <!-- https://w3id.org/icon/ontology/hasFactualMeaning -->

    <owl:NamedIndividual rdf:about="https://w3id.org/icon/ontology/hasFactualMeaning">
        <skos:broadMatch rdf:resource="http://erlangen-crm.org/current/P138_represents"/>
    </owl:NamedIndividual>
    


    <!-- https://w3id.org/icon/ontology/hasNamedObject -->

    <owl:NamedIndividual rdf:about="https://w3id.org/icon/ontology/hasNamedObject">
        <skos:broadMatch rdf:resource="http://erlangen-crm.org/current/P138_represents"/>
    </owl:NamedIndividual>
    


    <!-- https://w3id.org/icon/ontology/hasPersonification -->

    <owl:NamedIndividual rdf:about="https://w3id.org/icon/ontology/hasPersonification">
        <skos:broadMatch rdf:resource="http://erlangen-crm.org/current/P138_represents"/>
    </owl:NamedIndividual>
    


    <!-- https://w3id.org/icon/ontology/hasPlace -->

    <owl:NamedIndividual rdf:about="https://w3id.org/icon/ontology/hasPlace">
        <skos:broadMatch rdf:resource="http://erlangen-crm.org/current/P138_represents"/>
    </owl:NamedIndividual>
    


    <!-- https://w3id.org/icon/ontology/hasPrototypicalMotif -->

    <owl:NamedIndividual rdf:about="https://w3id.org/icon/ontology/hasPrototypicalMotif">
        <skos:broadMatch rdf:resource="http://w3id.org/vir#K4_is_visual_prototype_of"/>
    </owl:NamedIndividual>
    


    <!-- https://w3id.org/icon/ontology/hasSymbol -->

    <owl:NamedIndividual rdf:about="https://w3id.org/icon/ontology/hasSymbol">
        <skos:broadMatch rdf:resource="http://erlangen-crm.org/current/P138_represents"/>
    </owl:NamedIndividual>
    


    <!-- https://w3id.org/icon/ontology/recognizedArtisticMotif -->

    <owl:NamedIndividual rdf:about="https://w3id.org/icon/ontology/recognizedArtisticMotif">
        <skos:broadMatch rdf:resource="http://erlangen-crm.org/current/P141_assigned"/>
    </owl:NamedIndividual>
    


    <!-- https://w3id.org/icon/ontology/recognizedComposition -->

    <owl:NamedIndividual rdf:about="https://w3id.org/icon/ontology/recognizedComposition">
        <skos:broadMatch rdf:resource="http://erlangen-crm.org/current/P141_assigned"/>
    </owl:NamedIndividual>
    


    <!-- https://w3id.org/icon/ontology/recognizedImage -->

    <owl:NamedIndividual rdf:about="https://w3id.org/icon/ontology/recognizedImage">
        <skos:broadMatch rdf:resource="http://erlangen-crm.org/current/P141_assigned"/>
    </owl:NamedIndividual>
    


    <!-- https://w3id.org/icon/ontology/recognizedInvenzione -->

    <owl:NamedIndividual rdf:about="https://w3id.org/icon/ontology/recognizedInvenzione">
        <skos:broadMatch rdf:resource="http://erlangen-crm.org/current/P141_assigned"/>
    </owl:NamedIndividual>
    


    <!-- 
    ///////////////////////////////////////////////////////////////////////////////////////
    //
    // Annotations
    //
    ///////////////////////////////////////////////////////////////////////////////////////
     -->

    <rdf:Description rdf:about="http://iflastandards.info/ns/fr/frbr/frbroo/F38">
        <rdfs:label xml:lang="en">Character</rdfs:label>
    </rdf:Description>
    <rdf:Description rdf:about="https://w3id.org/icon/ontology/Action">
        <rdfs:comment xml:lang="en">An event as recognized at level 1 of interpretation, e.g. a man who lifts one hand or a man riding a horse. Generally, all the actions should be described by this class.  When an action is identified, it is suggested to create a Composition with all the elements involved in this action</rdfs:comment>
        <rdfs:isDefinedBy rdf:resource="https://w3id.org/icon/ontology/ICONOntology"/>
        <rdfs:label xml:lang="en">Action (ICON)</rdfs:label>
    </rdf:Description>
    <rdf:Description rdf:about="https://w3id.org/icon/ontology/Allegory">
        <rdfs:label xml:lang="en">Allegory</rdfs:label>
        <rdfs:isDefinedBy rdf:resource="https://w3id.org/icon/ontology/ICONOntology"/>
        <rdfs:comment xml:lang="en">An Allegory is a cohese combination of images that represent either symbols of personifications. Allegories are recognized in the context of iconographical recognition; their recognition can be included in an Iconographical Description. This definition of Allegory has been taken from Panofsky&apos;s Studies in Iconology (1939). Nevertheless, also a story can have a symbolical meaning. In this case, it is suggested to associate a Story to the images describing its content, an allegory  to the images describing the story and the symbolical meaning associated to it. E.g.: the fall of Phaeton was generally considered as an allegory of the fate of every temerarius (Panofsky 1939, p. 218). Therefore, the image identifying Phaeton is linked both to the Allegory and to the Story.</rdfs:comment>
    </rdf:Description>
    <rdf:Description rdf:about="https://w3id.org/icon/ontology/ArtisticMotif">
        <rdfs:isDefinedBy rdf:resource="https://w3id.org/icon/ontology/ICONOntology"/>
        <rdfs:comment xml:lang="en">An ArtisticMotif is the output of a Pre Iconographic Recognition. It is a N-ary relationship class linking the physical unique representation depicted in an artwork to the corresponding real world meaning recognized. Each artistic motif describes exactly one meaning among: Natural Element, Action, Expression Quality. Qualities (e.g. colors) can be expressed.
The N-ary structure allow first of all to maintain the distinction between the particular representation belonging to the artwork considered and the general meaning of which the representation is an expression. Furthermore, it allows to carefully describe in detail what is represented in the visual representation, since it gives the chance to identify uniquely details of objects and iconographies.</rdfs:comment>
        <rdfs:label xml:lang="en">Artistic Motif</rdfs:label>
    </rdf:Description>
    <rdf:Description rdf:about="https://w3id.org/icon/ontology/Artwork">
        <rdfs:label xml:lang="en">Artwork</rdfs:label>
        <rdfs:comment xml:lang="en">The artwork is a visual representation that may be relevant from an iconographical or an iconological point of view, carried by a physical cultural object (dul:InformationRealization) usually created by a person.</rdfs:comment>
        <rdfs:isDefinedBy rdf:resource="https://w3id.org/icon/ontology/ICONOntology"/>
    </rdf:Description>
    <rdf:Description rdf:about="https://w3id.org/icon/ontology/Character">
        <rdfs:label xml:lang="en">Character</rdfs:label>
        <rdfs:comment xml:lang="en">A Character is a real or imaginary being identifiable as a subject in the Iconographical Analysis (level 2 of interpretation)</rdfs:comment>
        <rdfs:isDefinedBy rdf:resource="https://w3id.org/icon/ontology/ICONOntology"/>
    </rdf:Description>
    <rdf:Description rdf:about="https://w3id.org/icon/ontology/Composition">
        <rdfs:comment xml:lang="en">A Composition is a jointly of ArtisticMotif having a meaning. It can be recognized as corresponding to the same image at the second level or interpretation, or can explicit groupings of level 1 elements that the descriptor considers significant. Its is suggested to express the level 1 elements involved every time that there is an action (e.g. the action &quot;lifting&quot; in the context of &quot;man lifting a woman&quot; should be grouped in a composition including the artistic motifs corresponding respectively to &quot;man&quot;, &quot;woman, &quot;lifting&quot;)</rdfs:comment>
        <rdfs:isDefinedBy rdf:resource="https://w3id.org/icon/ontology/ICONOntology"/>
        <rdfs:label xml:lang="en">Composition</rdfs:label>
    </rdf:Description>
    <rdf:Description rdf:about="https://w3id.org/icon/ontology/Event">
        <rdfs:isDefinedBy rdf:resource="https://w3id.org/icon/ontology/ICONOntology"/>
        <rdfs:comment xml:lang="en">An Event is an action that is depicted as subject by an artwork. It differs from the first level Action since it requires deeper interpretation to be identified. For example, the act of hurling the Trident (Action) held by Neptune in some iconographies is interpreted as the act of calming the storm (Event) provoked by Juno in Virgil&apos;s Aeneid book 1. Furthermore, an Event is linked to a icon:Image, and not to a icon:Artistic Motif. This class includes also events having a proper identity, such as historical events (e.g. the Battle of Cascina).</rdfs:comment>
        <rdfs:label xml:lang="en">Event</rdfs:label>
    </rdf:Description>
    <rdf:Description rdf:about="https://w3id.org/icon/ontology/ExpressionalQuality">
        <rdfs:label xml:lang="en">Expressional Quality</rdfs:label>
        <rdfs:isDefinedBy rdf:resource="https://w3id.org/icon/ontology/ICONOntology"/>
        <rdfs:comment xml:lang="en">An Expression Quality corresponds to the &quot;expressional subject matter&quot; described by Panofsky (1939), which belongs, along with the factual ones, to the Primary or natural subject matter of a work of art. Indeed, it individuates, by way of example, emotions, an atmosphere, the character of a person.</rdfs:comment>
    </rdf:Description>
    <rdf:Description rdf:about="https://w3id.org/icon/ontology/Image">
        <rdfs:isDefinedBy rdf:resource="https://w3id.org/icon/ontology/ICONOntology"/>
        <rdfs:label xml:lang="en">Image</rdfs:label>
        <rdfs:comment xml:lang="en">Image is a reification class linking the identified second level subject (namely: Characters, Events, Places, Named Objects, Symbols and Personifications) to the specific interpretation that recognizes it. It represents the subject depicted as a manifestation in the specific artwork taken into account, in contrast to the second level subjects cited and Invenzione, identifying iconographies from an abstract and general point of view. This distinction between the general subject level and the artwork-specific one is functional to identify the variants of a subject in relation to the specific context.</rdfs:comment>
    </rdf:Description>
    <rdf:Description rdf:about="https://w3id.org/icon/ontology/InterpretationDescription">
        <rdfs:isDefinedBy rdf:resource="https://w3id.org/icon/ontology/ICONOntology"/>
        <rdfs:label xml:lang="en">Interpretation Description</rdfs:label>
        <rdfs:comment xml:lang="en">The Interpretation Description is a class collecting all the triples describing each recognition in each level that shares a unique interpretative perspective. For example, it allows to collect claims agreeing each other or to describe the situation in which an art historian attributes to other art historians some details of the general interpretation he claims. Recognitions in disagree with each other should be documented in different descriptions. For example, the interpretation made in 1699 recognising Regnaudin&apos;s statuette as depicting &quot;Time carrying off the Truth&quot; is listed in a different description form the interpretation recognising &quot;The rape of Cybele&quot; as its subject (Wittkower).</rdfs:comment>
    </rdf:Description>
    <rdf:Description rdf:about="https://w3id.org/icon/ontology/IntrinsicMeaning">
        <rdfs:comment xml:lang="en">N-ary relatioship class linking the identified cultural phenomenon or deeper meaning to the whole artwork or to the specific part of its representation and to the interpretation that identifies it. From a theoretical point of view, it corresponds to the manifestation in the specific artwork of the concepts and cultural phenomena identified by the iconological analysis. The terminology is taken from Panofsky (1939, 1955).</rdfs:comment>
        <rdfs:isDefinedBy rdf:resource="https://w3id.org/icon/ontology/ICONOntology"/>
        <rdfs:label xml:lang="en">Intrinsic Meaning</rdfs:label>
    </rdf:Description>
    <rdf:Description rdf:about="https://w3id.org/icon/ontology/Invenzione">
        <rdfs:comment xml:lang="en">An Invenzione, term taken from Panofsky&apos;s Studies in Iconology (1939), is the subject matter represented by the combination of the single images recognized. The recognition of an Invenzione happens in the context of the iconographical recognition and it is included in the Iconographical Description. This definition slightly differs from the Panofsky&apos;s one: while he describes an invenzione as a form expressing the subject, we consider it as an individual belonging to the &quot;sphere of secondary or conventional subject matter, viz., the world of specific themes or concepts manifested in images [...]&quot;. This new definition has been introduced to allow to formalize and recognize subjects represented in different artworks. Nevertheless, the identity of form and subject is already included in the definition of the class Artwork. Story and Allegory are subclasses of Invenzione.</rdfs:comment>
        <rdfs:isDefinedBy rdf:resource="https://w3id.org/icon/ontology/ICONOntology"/>
        <rdfs:label xml:lang="en">Invenzione</rdfs:label>
    </rdf:Description>
    <rdf:Description rdf:about="https://w3id.org/icon/ontology/NamedObject">
        <rdfs:isDefinedBy rdf:resource="https://w3id.org/icon/ontology/ICONOntology"/>
        <rdfs:comment xml:lang="en">A named object is a non-living unique element that is often used as an attribute for the recognition of specific characters or as the individuals of a more general concept class. (e.g. Bible for the Book class)</rdfs:comment>
        <rdfs:label xml:lang="en">Named Object</rdfs:label>
    </rdf:Description>
    <rdf:Description rdf:about="https://w3id.org/icon/ontology/NaturalElement">
        <rdfs:comment xml:lang="en">Comprises objects, human beings, natural elements that can be experienced. They are recognized at the first level of interpretation.</rdfs:comment>
        <rdfs:label xml:lang="en">Natural Element</rdfs:label>
        <rdfs:isDefinedBy rdf:resource="https://w3id.org/icon/ontology/ICONOntology"/>
    </rdf:Description>
    <rdf:Description rdf:about="https://w3id.org/icon/ontology/Personification">
        <rdfs:isDefinedBy rdf:resource="https://w3id.org/icon/ontology/ICONOntology"/>
        <rdfs:label xml:lang="en">Personification (ICON)</rdfs:label>
        <rdfs:comment xml:lang="en">A representation of a concept through a human figure</rdfs:comment>
    </rdf:Description>
    <rdf:Description rdf:about="https://w3id.org/icon/ontology/Place">
        <rdfs:comment xml:lang="en">An identified setting, e.g. the city of Bologna, which is recognized as a Level 2 subject. The recognition of a generic city is formally represented by the Natural Element class (level 1).</rdfs:comment>
        <rdfs:label xml:lang="en">Place (ICON)</rdfs:label>
        <rdfs:isDefinedBy rdf:resource="https://w3id.org/icon/ontology/ICONOntology"/>
    </rdf:Description>
    <rdf:Description rdf:about="https://w3id.org/icon/ontology/Recognition">
        <rdfs:comment xml:lang="en">A recognition, in the context of this ontology, is an interpretation act made by an agent (biological or electronic being) that links works of arts to something related to their content. More specific recognitions are available as subclasses for specific types of recognition according to the level of interpretation.</rdfs:comment>
        <rdfs:label xml:lang="en">Recognition</rdfs:label>
        <rdfs:isDefinedBy rdf:resource="https://w3id.org/icon/ontology/ICONOntology"/>
    </rdf:Description>
    <rdf:Description rdf:about="https://w3id.org/icon/ontology/Story">
        <rdfs:isDefinedBy rdf:resource="https://w3id.org/icon/ontology/ICONOntology"/>
        <rdfs:label xml:lang="en">Story</rdfs:label>
        <rdfs:comment xml:lang="en">A story is a cohese combination of images that represent narrative elements such as Characters, Places, Events, Named Objects. The recognition of a story happens in the context of an Iconographical Recognition, and it is included in an Iconographical Description. As the super class Invenzione, it concerns the word of the subject matter. It is not necessary to have multiple images to compose a story.</rdfs:comment>
    </rdf:Description>
    <rdf:Description rdf:about="https://w3id.org/icon/ontology/Symbol">
        <rdfs:isDefinedBy rdf:resource="https://w3id.org/icon/ontology/ICONOntology"/>
        <rdfs:label xml:lang="en">Symbol</rdfs:label>
        <rdfs:comment xml:lang="en">A Symbol is the class representing the unity of a symbol and its symbolic meaning that can be expressed by an Image. The represented object (Simulacrum) and the symbolical meaning expressed (Reality Counterpart) along with the type of relation linking them if further represented by the Simulation Ontology.</rdfs:comment>
    </rdf:Description>
    <rdf:Description rdf:about="https://w3id.org/icon/ontology/hasCharacter">
        <rdfs:label xml:lang="en">Has Character</rdfs:label>
        <rdfs:isDefinedBy rdf:resource="https://w3id.org/icon/ontology/ICONOntology"/>
        <rdfs:comment xml:lang="en">This relation links an image to the Character depicted</rdfs:comment>
    </rdf:Description>
    <rdf:Description rdf:about="https://w3id.org/icon/ontology/hasCopiedMotif">
        <rdfs:isDefinedBy rdf:resource="https://w3id.org/icon/ontology/ICONOntology"/>
        <rdfs:label xml:lang="en">Has Copied Motif</rdfs:label>
        <rdfs:comment xml:lang="en">This relation associates to the act of Formal Motif Recognition the Artistic Motif representing the copied visual pattern. To be used when it is affirmed that a specific feature has as a prototype the same feature of a specific visual item.</rdfs:comment>
    </rdf:Description>
    <rdf:Description rdf:about="https://w3id.org/icon/ontology/hasEvent">
        <rdfs:isDefinedBy rdf:resource="https://w3id.org/icon/ontology/ICONOntology"/>
        <rdfs:comment xml:lang="en">This relation links an image to the Event depicted</rdfs:comment>
        <rdfs:label xml:lang="en">Has Event</rdfs:label>
    </rdf:Description>
    <rdf:Description rdf:about="https://w3id.org/icon/ontology/hasExpressionalMeaning">
        <rdfs:label xml:lang="en">Has Expressional Meaning</rdfs:label>
        <rdfs:comment>This relation links the Expressional Meaning recognized to the Artistic Motif</rdfs:comment>
        <rdfs:isDefinedBy rdf:resource="https://w3id.org/icon/ontology/ICONOntology"/>
    </rdf:Description>
    <rdf:Description rdf:about="https://w3id.org/icon/ontology/hasFactualMeaning">
        <rdfs:isDefinedBy rdf:resource="https://w3id.org/icon/ontology/ICONOntology"/>
        <rdfs:comment>This relation links the Factual Meaning recognized (Actions or Natural Elements) to the Artistic Motif</rdfs:comment>
        <rdfs:label xml:lang="en">Has Factual Meaning</rdfs:label>
    </rdf:Description>
    <rdf:Description rdf:about="https://w3id.org/icon/ontology/hasNamedObject">
        <rdfs:isDefinedBy rdf:resource="https://w3id.org/icon/ontology/ICONOntology"/>
        <rdfs:label xml:lang="en">Has Named Object</rdfs:label>
        <rdfs:comment xml:lang="en">This relation links an image to the Named Object depicted</rdfs:comment>
    </rdf:Description>
    <rdf:Description rdf:about="https://w3id.org/icon/ontology/hasPersonification">
        <rdfs:comment xml:lang="en">This relation links an image to the Personification depicted</rdfs:comment>
        <rdfs:label xml:lang="en">Has Personification</rdfs:label>
        <rdfs:isDefinedBy rdf:resource="https://w3id.org/icon/ontology/ICONOntology"/>
    </rdf:Description>
    <rdf:Description rdf:about="https://w3id.org/icon/ontology/hasPlace">
        <rdfs:comment xml:lang="en">This relation links an image to the Place depicted</rdfs:comment>
        <rdfs:isDefinedBy rdf:resource="https://w3id.org/icon/ontology/ICONOntology"/>
        <rdfs:label xml:lang="en">Has Place</rdfs:label>
    </rdf:Description>
    <rdf:Description rdf:about="https://w3id.org/icon/ontology/hasPrototypicalMotif">
        <rdfs:comment xml:lang="en">This relation associates to the act of the Recognition of a formal motif to the artistic motif from which the visual pattern derives. It should be used when it is affirmed that a specific feature has as a prototype the same feature of a specific visual item.</rdfs:comment>
        <rdfs:label xml:lang="en">Has Prototypical Motif</rdfs:label>
        <rdfs:isDefinedBy rdf:resource="https://w3id.org/icon/ontology/ICONOntology"/>
    </rdf:Description>
    <rdf:Description rdf:about="https://w3id.org/icon/ontology/hasSymbol">
        <rdfs:comment xml:lang="en">This relation links an image to the Symbol depicted</rdfs:comment>
        <rdfs:label xml:lang="en">Has Symbol</rdfs:label>
        <rdfs:isDefinedBy rdf:resource="https://w3id.org/icon/ontology/ICONOntology"/>
    </rdf:Description>
    <rdf:Description rdf:about="https://w3id.org/icon/ontology/recognizedArtisticMotif">
        <rdfs:label xml:lang="en">Recognized Artistic Motif</rdfs:label>
        <rdfs:isDefinedBy rdf:resource="https://w3id.org/icon/ontology/ICONOntology"/>
        <rdfs:comment xml:lang="en">This relation associates the Artistic Motif to the Pre-iconographical Recognition that recognizes it at the first level of interpretation.</rdfs:comment>
    </rdf:Description>
    <rdf:Description rdf:about="https://w3id.org/icon/ontology/recognizedComposition">
        <rdfs:isDefinedBy rdf:resource="https://w3id.org/icon/ontology/ICONOntology"/>
        <rdfs:comment xml:lang="en">This relation associates the Composition to the Pre-iconographical Recognition that recognizes it at the first level of interpretation.</rdfs:comment>
        <rdfs:label xml:lang="en">Recognized Composition</rdfs:label>
    </rdf:Description>
    <rdf:Description rdf:about="https://w3id.org/icon/ontology/recognizedImage">
        <rdfs:isDefinedBy rdf:resource="https://w3id.org/icon/ontology/ICONOntology"/>
        <rdfs:comment xml:lang="en">This relation associates the Image to the Iconographical Recognition that recognizes it at the second level of interpretation.</rdfs:comment>
        <rdfs:label xml:lang="en">Recognized Image</rdfs:label>
    </rdf:Description>
    <rdf:Description rdf:about="https://w3id.org/icon/ontology/recognizedInvenzione">
        <rdfs:comment xml:lang="en">This relation associates the Invenzione to the Iconographical Recognition that recognizes it at the second level of interpretation.</rdfs:comment>
        <rdfs:isDefinedBy rdf:resource="https://w3id.org/icon/ontology/ICONOntology"/>
        <rdfs:label xml:lang="en">Recognized Invenzione</rdfs:label>
    </rdf:Description>
</rdf:RDF>



<!-- Generated by the OWL API (version 4.5.9.2019-02-01T07:24:44Z) https://github.com/owlcs/owlapi -->

